more adapting

Weidenbach_Book/CDCL_W_Implementation.thy
@@ -1,17 +1,16 @@
 theory CDCL_W_Implementation
-imports DPLL_CDCL_W_Implementation CDCL_W_Abstract_State
+imports DPLL_CDCL_W_Implementation CDCL_W_Termination
 begin
 
 subsubsection \<open>Types and Instantiation\<close>
 notation image_mset (infixr "`#" 90)
 
-type_synonym 'a cdcl\<^sub>W_mark = "'a literal list"
+type_synonym 'a cdcl\<^sub>W_mark = "'a clause"
 
-type_synonym 'v cdcl\<^sub>W_ann_lit = "('v,  'v cdcl\<^sub>W_mark) ann_lit"
+type_synonym 'v cdcl\<^sub>W_ann_lit = "('v, 'v cdcl\<^sub>W_mark) ann_lit"
 type_synonym 'v cdcl\<^sub>W_ann_lits = "('v, 'v cdcl\<^sub>W_mark) ann_lits"
 type_synonym 'v cdcl\<^sub>W_state =
-  "'v cdcl\<^sub>W_ann_lits \<times> 'v literal list list \<times> 'v literal list list \<times> nat \<times>
-  'v literal list option"
+  "'v cdcl\<^sub>W_ann_lits \<times> 'v clauses \<times> 'v clauses \<times> nat \<times> 'v clause option"
 
 abbreviation raw_trail :: "'a \<times> 'b \<times> 'c \<times> 'd \<times> 'e \<Rightarrow> 'a" where
 "raw_trail \<equiv> (\<lambda>(M, _). M)"
@@ -43,149 +42,91 @@ abbreviation raw_update_conflicting :: "'e \<Rightarrow> 'a \<times> 'b \<times>
   where
 "raw_update_conflicting \<equiv> \<lambda>S (M, N, U, k, _).  (M, N, U, k, S)"
 
-abbreviation raw_add_learned_cls where
-"raw_add_learned_cls \<equiv> \<lambda>C (M, N, U, S). (M, N, {#C#} + U, S)"
+abbreviation "S0_cdcl\<^sub>W N \<equiv> (([], N, {#}, 0, None):: 'v cdcl\<^sub>W_state)"
+
+abbreviation raw_add_learned_clss where
+"raw_add_learned_clss \<equiv> \<lambda>C (M, N, U, S). (M, N, {#C#} + U, S)"
 
 abbreviation raw_remove_cls where
 "raw_remove_cls \<equiv> \<lambda>C (M, N, U, S). (M, removeAll_mset C N, removeAll_mset C U, S)"
 
-type_synonym 'v cdcl\<^sub>W_state_inv_st = "('v, 'v literal list) ann_lits \<times>
-  'v literal list list \<times> 'v literal list list \<times> nat \<times> 'v literal list option"
+lemma raw_trail_conv: "raw_trail (M, N, U, k, D) = M" and
+  clauses_conv: "raw_init_clss (M, N, U, k, D) = N" and
+  raw_learned_clss_conv: "raw_learned_clss (M, N, U, k, D) = U" and
+  raw_conflicting_conv: "raw_conflicting (M, N, U, k, D) = D" and
+  raw_backtrack_lvl_conv: "raw_backtrack_lvl (M, N, U, k, D) = k"
+  by auto
 
-abbreviation "raw_S0_cdcl\<^sub>W N \<equiv> (([], N, [], 0, None):: 'v cdcl\<^sub>W_state_inv_st)"
-
-fun mmset_of_mlit' :: "('v, 'v literal list) ann_lit \<Rightarrow> ('v, 'v clause) ann_lit"
-  where
-"mmset_of_mlit' (Propagated L C) = Propagated L (mset C)" |
-"mmset_of_mlit' (Decided L) = Decided L"
-
-lemma lit_of_mmset_of_mlit'[simp]:
-  "lit_of (mmset_of_mlit' xa) = lit_of xa"
-  by (induction xa) auto
-
-abbreviation trail where
-"trail S \<equiv> map mmset_of_mlit' (raw_trail S)"
-
-abbreviation clauses_of_l where
-"clauses_of_l \<equiv> \<lambda>L. mset (map mset L)"
+lemma state_conv:
+  "S = (raw_trail S, raw_init_clss S, raw_learned_clss S, raw_backtrack_lvl S, raw_conflicting S)"
+  by (cases S) auto
 
 
-fun reduce_trail_to where
-"reduce_trail_to M1 S =
-  (case S of
-    (M, N, U, k, C) \<Rightarrow> (drop (length M - length M1) M, N, U, k, C))"
-
-    
-global_interpretation abs_state\<^sub>W_ops
-  "mset::'v literal list \<Rightarrow> 'v clause"
-
-  clauses_of_l "op @" "\<lambda>L C. L \<in> set C" "op #" "\<lambda>C. remove1_cond (\<lambda>L. mset L = mset C)"
-
-  mset "\<lambda>xs ys. case_prod append (fold (\<lambda>x (ys, zs). (remove1 x ys, x # zs)) xs (ys, []))"
-  remove1
-
-  id id
-
-  "\<lambda>(M, _). map mmset_of_mlit' M" "\<lambda>(M, _). hd M"
-  "\<lambda>(_, N, _). N"
-  "\<lambda>(_, _, U, _). U"
-  "\<lambda>(_, _, _, k, _). k"
-  "\<lambda>(_, _, _, _, C). C"
-
+interpretation state\<^sub>W 
+  raw_trail raw_init_clss raw_learned_clss raw_backtrack_lvl raw_conflicting
   "\<lambda>L (M, S). (L # M, S)"
   "\<lambda>(M, S). (tl M, S)"
-  "\<lambda>C (M, N, U, S). (M, N, C # U, S)"
-  "\<lambda>C (M, N, U, S). (M, filter (\<lambda>L. mset L \<noteq> mset C) N, filter (\<lambda>L. mset L \<noteq> mset C) U, S)"
+  "\<lambda>C (M, N, U, S). (M, N, {#C#} + U, S)"
+  "\<lambda>C (M, N, U, S). (M, removeAll_mset C N, removeAll_mset C U, S)"
   "\<lambda>(k::nat) (M, N, U, _, D). (M, N, U, k, D)"
   "\<lambda>D (M, N, U, k, _). (M, N, U, k, D)"
-  reduce_trail_to
-  "\<lambda>N. ([], N, [], 0, None)"
+  "\<lambda>N. ([], N, {#}, 0, None)"
   "\<lambda>(_, N, U, _). ([], N, U, 0, None)"
-  apply unfold_locales by (auto simp: hd_map comp_def map_tl ac_simps
-    union_mset_list mset_map_mset_remove1_cond ex_mset)
+  by unfold_locales auto
 
-lemma mmset_of_mlit'_mmset_of_mlit: "mmset_of_mlit' = mmset_of_mlit"
-  apply (rule ext)
-  apply (case_tac x)
-  apply auto
-  done
-
-lemma clauses_of_l_filter_removeAll:
-  "clauses_of_l [L\<leftarrow>a . mset L \<noteq> mset C] = mset (removeAll (mset C) (map mset a))"
-  by (induct a) auto
-lemma map_drop_reduce_trail_to:
-  "map mmset_of_mlit a = M2 @ M1 \<Longrightarrow> map mmset_of_mlit (drop (length a - length M1) a) = M1"
-   by (metis add_diff_cancel_right' cancel_comm_monoid_add_class.diff_cancel drop_0 drop_all
-     drop_append drop_map length_append length_map order_refl self_append_conv2)
-
-interpretation abs_state\<^sub>W
-  "mset::'v literal list \<Rightarrow> 'v clause"
-
-  clauses_of_l "op @" "\<lambda>L C. L \<in> set C" "op #" "\<lambda>C. remove1_cond (\<lambda>L. mset L = mset C)"
-
-  mset "\<lambda>xs ys. case_prod append (fold (\<lambda>x (ys, zs). (remove1 x ys, x # zs)) xs (ys, []))"
-  remove1
-
-  id id
-
-  "\<lambda>(M, _). map mmset_of_mlit' M" "\<lambda>(M, _). hd M"
-  "\<lambda>(_, N, _). N"
-  "\<lambda>(_, _, U, _). U"
-  "\<lambda>(_, _, _, k, _). k"
-  "\<lambda>(_, _, _, _, C). C"
-
+interpretation conflict_driven_clause_learning\<^sub>W raw_trail raw_init_clss raw_learned_clss raw_backtrack_lvl raw_conflicting
   "\<lambda>L (M, S). (L # M, S)"
   "\<lambda>(M, S). (tl M, S)"
-  "\<lambda>C (M, N, U, S). (M, N, C # U, S)"
-  "\<lambda>C (M, N, U, S). (M, filter (\<lambda>L. mset L \<noteq> mset C) N, filter (\<lambda>L. mset L \<noteq> mset C) U, S)"
+  "\<lambda>C (M, N, U, S). (M, N, {#C#} + U, S)"
+  "\<lambda>C (M, N, U, S). (M, removeAll_mset C N, removeAll_mset C U, S)"
   "\<lambda>(k::nat) (M, N, U, _, D). (M, N, U, k, D)"
   "\<lambda>D (M, N, U, k, _). (M, N, U, k, D)"
-  reduce_trail_to
-  "\<lambda>N. ([], N, [], 0, None)"
+  "\<lambda>N. ([], N, {#}, 0, None)"
   "\<lambda>(_, N, U, _). ([], N, U, 0, None)"
-  apply unfold_locales
-  apply (rename_tac S, case_tac S)
-  by (auto simp: hd_map comp_def map_tl ac_simps clauses_of_l_filter_removeAll
-    mmset_of_mlit'_mmset_of_mlit map_drop_reduce_trail_to)
+  by unfold_locales auto
 
-global_interpretation abs_conflict_driven_clause_learning\<^sub>W
-  "mset::'v literal list \<Rightarrow> 'v clause"
+declare clauses_def[simp]
 
-  clauses_of_l "op @" "\<lambda>L C. L \<in> set C" "op #" "\<lambda>C. remove1_cond (\<lambda>L. mset L = mset C)"
+lemma cdcl\<^sub>W_state_eq_equality[iff]: "state_eq S T \<longleftrightarrow> S = T"
+  unfolding state_eq_def by (cases S, cases T) auto
+declare state_simp[simp del]
 
-  mset "\<lambda>xs ys. case_prod append (fold (\<lambda>x (ys, zs). (remove1 x ys, x # zs)) xs (ys, []))"
-  remove1
+lemma reduce_trail_to_empty_trail[simp]:
+  "reduce_trail_to F ([], aa, ab, ac, b) = ([], aa, ab, ac, b)"
+  using reduce_trail_to.simps by auto
 
-  id id
+lemma raw_trail_reduce_trail_to_length_le:
+  assumes "length F > length (raw_trail S)"
+  shows "raw_trail (reduce_trail_to F S) = []"
+  using assms trail_reduce_trail_to_length_le[of S F]
+  by (cases S, cases "reduce_trail_to F S") auto
 
-  "\<lambda>(M, _). map mmset_of_mlit' M" "\<lambda>(M, _). hd M"
-  "\<lambda>(_, N, _). N"
-  "\<lambda>(_, _, U, _). U"
-  "\<lambda>(_, _, _, k, _). k"
-  "\<lambda>(_, _, _, _, C). C"
-
-  "\<lambda>L (M, S). (L # M, S)"
-  "\<lambda>(M, S). (tl M, S)"
-  "\<lambda>C (M, N, U, S). (M, N, C # U, S)"
-  "\<lambda>C (M, N, U, S). (M, filter (\<lambda>L. mset L \<noteq> mset C) N, filter (\<lambda>L. mset L \<noteq> mset C) U, S)"
-  "\<lambda>(k::nat) (M, N, U, _, D). (M, N, U, k, D)"
-  "\<lambda>D (M, N, U, k, _). (M, N, U, k, D)"
-  reduce_trail_to
-  "\<lambda>N. ([], N, [], 0, None)"
-  "\<lambda>(_, N, U, _). ([], N, U, 0, None)"
-  by intro_locales
-
-declare state_simp[simp del] raw_clauses_def[simp]
-notation state_eq (infix "\<sim>" 50)
-term reduce_trail_to
-
-lemma reduce_trail_to_map[simp]:
-  "reduce_trail_to (map f M1) = reduce_trail_to M1"
-  by (rule ext) (auto intro:)
+lemma reduce_trail_to:
+  "reduce_trail_to F S =
+    ((if length (raw_trail S) \<ge> length F
+    then drop (length (raw_trail S) - length F) (raw_trail S)
+    else []), raw_init_clss S, raw_learned_clss S, raw_backtrack_lvl S, raw_conflicting S)"
+    (is "?S = _")
+proof (induction F S rule: reduce_trail_to.induct)
+  case (1 F S) note IH = this
+  show ?case
+    proof (cases "raw_trail S")
+      case Nil
+      then show ?thesis using IH by (cases S) auto
+    next
+      case (Cons L M)
+      then show ?thesis
+        apply (cases "Suc (length M) > length F")
+         prefer 2 using IH reduce_trail_to_length_ne[of S F] apply (cases S) apply auto[]
+        apply (subgoal_tac "Suc (length M) - length F = Suc (length M - length F)")
+        using reduce_trail_to_length_ne[of S F] IH by (cases S) auto
+    qed
+qed
 
 subsection \<open>CDCL Implementation\<close>
-subsubsection \<open>Types and Additional Lemmas\<close>
-lemma true_clss_remdups[simp]:
+subsubsection \<open>Definition of the rules\<close>
+paragraph \<open>Types\<close>
+lemma true_raw_init_clss_remdups[simp]:
   "I \<Turnstile>s (mset \<circ> remdups) ` N \<longleftrightarrow>  I \<Turnstile>s mset ` N"
   by (simp add: true_clss_def)
 
@@ -193,42 +134,46 @@ lemma satisfiable_mset_remdups[simp]:
   "satisfiable ((mset \<circ> remdups) ` N) \<longleftrightarrow> satisfiable (mset ` N)"
 unfolding satisfiable_carac[symmetric] by simp
 
-text \<open>We need some functions to convert between our abstract state @{typ "nat cdcl\<^sub>W_state"} and the
+
+type_synonym 'v cdcl\<^sub>W_state_inv_st = "('v, 'v literal list) ann_lit list \<times>
+  'v literal list list \<times> 'v literal list list \<times> nat \<times> 'v literal list option"
+
+text \<open>We need some functions to convert between our abstract state @{typ "'v cdcl\<^sub>W_state"} and the
  concrete state @{typ "'v cdcl\<^sub>W_state_inv_st"}.\<close>
+
+fun convert :: "('a, 'c list) ann_lit \<Rightarrow> ('a, 'c multiset) ann_lit"  where
+"convert (Propagated L C) = Propagated L (mset C)" |
+"convert (Decided K) = Decided K"
 
 abbreviation convertC :: "'a list option \<Rightarrow> 'a multiset option"  where
 "convertC \<equiv> map_option mset"
 
 lemma convert_Propagated[elim!]:
-  "mmset_of_mlit' z = Propagated L C \<Longrightarrow> (\<exists>C'. z = Propagated L C' \<and> C = mset C')"
+  "convert z = Propagated L C \<Longrightarrow> (\<exists>C'. z = Propagated L C' \<and> C = mset C')"
   by (cases z) auto
 
-lemma is_decided_mmset_of_mlit'[simp]: "is_decided (mmset_of_mlit' x) = is_decided x"
+lemma is_decided_convert[simp]: "is_decided (convert x) = is_decided x"
   by (cases x) auto
 
 lemma get_level_map_convert[simp]:
-  "get_level (map mmset_of_mlit' M) x = get_level M x"
+  "get_level (map convert M) x = get_level M x"
   by (induction M rule: ann_lit_list_induct) (auto simp: comp_def)
 
-lemma get_rev_level_map_mmsetof_mlit[simp]:
-  "get_level (map mmset_of_mlit' M) = get_level M"
-  by (induction M rule: ann_lit_list_induct) (auto intro!: ext simp: comp_def)
-
 lemma get_maximum_level_map_convert[simp]:
-  "get_maximum_level (map mmset_of_mlit' M) D = get_maximum_level M D"
-  by (induction D) (auto simp add: get_maximum_level_plus)
+  "get_maximum_level (map convert M) D = get_maximum_level M D"
+  by (induction D)
+     (auto simp add: get_maximum_level_plus)
 
-lemma reduce_trail_to_empty_trail[simp]:
-  "reduce_trail_to F ([], aa, ab, ac, b) = ([], aa, ab, ac, b)"
-  using reduce_trail_to.simps by auto
+text \<open>Conversion function\<close>
+fun toS :: "'v cdcl\<^sub>W_state_inv_st \<Rightarrow> 'v cdcl\<^sub>W_state" where
+"toS (M, N, U, k, C) = (map convert M, mset (map mset N),  mset (map mset U), k, convertC C)"
 
 text \<open>Definition an abstract type\<close>
-typedef 'v  cdcl\<^sub>W_state_inv = "{S::'v cdcl\<^sub>W_state_inv_st. cdcl\<^sub>W_mset.cdcl\<^sub>W_all_struct_inv (state S)}"
+typedef 'v cdcl\<^sub>W_state_inv =  "{S::'v cdcl\<^sub>W_state_inv_st. cdcl\<^sub>W_all_struct_inv (toS S)}"
   morphisms rough_state_of state_of
 proof
-  show "([],[], [], 0, None) \<in> ?cdcl\<^sub>W_state_inv"
-    unfolding cdcl\<^sub>W_mset.cdcl\<^sub>W_all_struct_inv_def
-    by (simp add: state_conc_init_state)
+  show "([],[], [], 0, None) \<in> {S. cdcl\<^sub>W_all_struct_inv (toS S)}"
+    by (auto simp add: cdcl\<^sub>W_all_struct_inv_def)
 qed
 
 instantiation cdcl\<^sub>W_state_inv :: (type) equal
@@ -239,25 +184,30 @@ instance
   by standard (simp add: rough_state_of_inject equal_cdcl\<^sub>W_state_inv_def)
 end
 
-lemma lits_of_map_convert[simp]: "lits_of_l (map mmset_of_mlit' M) = lits_of_l M"
+lemma lits_of_map_convert[simp]: "lits_of_l (map convert M) = lits_of_l M"
   by (induction M rule: ann_lit_list_induct) simp_all
 
+lemma atm_lit_of_convert[simp]:
+  "lit_of (convert x) =  lit_of x"
+  by (cases x) auto
+
 lemma undefined_lit_map_convert[iff]:
-  "undefined_lit (map mmset_of_mlit' M) L \<longleftrightarrow> undefined_lit M L"
-  by (auto simp add: defined_lit_map image_image mmset_of_mlit'_mmset_of_mlit)
+  "undefined_lit (map convert M) L \<longleftrightarrow> undefined_lit M L"
+  by (auto simp add: defined_lit_map image_image)
 
-lemma true_annot_map_convert[simp]: "map mmset_of_mlit' M \<Turnstile>a N \<longleftrightarrow> M \<Turnstile>a N"
-  by (induction M rule: ann_lit_list_induct) (simp_all add: true_annot_def
-    mmset_of_mlit'_mmset_of_mlit lits_of_def)
+lemma true_annot_map_convert[simp]: "map convert M \<Turnstile>a N \<longleftrightarrow> M \<Turnstile>a N"
+  by (simp_all add: true_annot_def image_image lits_of_def)
 
-lemma true_annots_map_convert[simp]: "map mmset_of_mlit' M \<Turnstile>as N \<longleftrightarrow> M \<Turnstile>as N"
+lemma true_annots_map_convert[simp]: "map convert M \<Turnstile>as N \<longleftrightarrow> M \<Turnstile>as N"
   unfolding true_annots_def by auto
 
+lemmas propagateE
 lemma find_first_unit_clause_some_is_propagate:
   assumes H: "find_first_unit_clause (N @ U) M = Some (L, C)"
-  shows "propagate_abs (M, N, U, k, None) (Propagated L C # M, N, U, k, None)"
+  shows "propagate (toS (M, N, U, k, None)) (toS (Propagated L C # M, N, U, k, None))"
   using assms
-  by (auto dest!: find_first_unit_clause_some intro!: propagate_abs_rule simp: raw_clauses_def)
+  by (auto dest!: find_first_unit_clause_some simp add: propagate.simps
+    intro!: exI[of _ "mset C - {#L#}"])
 
 subsubsection \<open>The Transitions\<close>
 paragraph \<open>Propagate\<close>
@@ -271,47 +221,62 @@ definition do_propagate_step where
   | S \<Rightarrow> S)"
 
 lemma do_propgate_step:
-  "do_propagate_step S \<noteq> S \<Longrightarrow> propagate_abs S (do_propagate_step S)"
-  apply (cases S, cases "conc_conflicting S")
-  using find_first_unit_clause_some_is_propagate[of "raw_init_clss S" "raw_learned_clss S"]
+  "do_propagate_step S \<noteq> S \<Longrightarrow> propagate (toS S) (toS (do_propagate_step S))"
+  apply (cases S, cases "raw_conflicting S")
+  using find_first_unit_clause_some_is_propagate[of "raw_init_clss S" "raw_learned_clss S" "raw_trail S" _ _
+    "raw_backtrack_lvl S"]
   by (auto simp add: do_propagate_step_def split: option.splits)
 
 lemma do_propagate_step_option[simp]:
-  "conc_conflicting S \<noteq> None \<Longrightarrow> do_propagate_step S = S"
-  unfolding do_propagate_step_def by (cases S, cases "conc_conflicting S") auto
-thm prod_cases
+  "raw_conflicting S \<noteq> None \<Longrightarrow> do_propagate_step S = S"
+  unfolding do_propagate_step_def by (cases S, cases "raw_conflicting S") auto
 
 lemma do_propagate_step_no_step:
-  assumes dist: "\<forall>c\<in>set (raw_clauses S). distinct c" and
+  assumes dist: "\<forall>c\<in>set (raw_init_clss S @ raw_learned_clss S). distinct c" and
   prop_step: "do_propagate_step S = S"
-  shows "no_step propagate_abs S"
+  shows "no_step propagate (toS S)"
 proof (standard, standard)
   fix T
-  assume "propagate_abs S T"
-  then obtain C L where
-    toSS: "conc_conflicting S = None" and
-    C: "C \<in> set (raw_clauses S)" and
-    L: "L \<in> set C" and
-    MC: "raw_trail S \<Turnstile>as CNot (mset (remove1 L C))" and
-    T: "T \<sim> raw_cons_trail (Propagated L C) S" and
-    undef: "undefined_lit (raw_trail S) L"
-    apply (cases S rule: prod_cases5)
-    by (elim propagate_absE) simp
+  assume "propagate (toS S) T"
+  then obtain M N U k C L E where
+    toSS: "toS S = (M, N, U, k, None)" and
+    LE: "L \<in># E" and
+    T: "T = (Propagated L E # M, N, U, k, None)" and
+    MC: "M \<Turnstile>as CNot C" and
+    undef: "undefined_lit M L" and
+    CL: "C + {#L#} \<in># N + U"
+    apply - by (cases "toS S") (auto elim!: propagateE)
   let ?M = "raw_trail S"
   let ?N = "raw_init_clss S"
   let ?U = "raw_learned_clss S"
   let ?k = "raw_backtrack_lvl S"
   let ?D = "None"
   have S: "S = (?M, ?N, ?U, ?k, ?D)"
-    using toSS by (cases S, cases "conc_conflicting S") simp_all
+    using toSS by (cases S, cases "raw_conflicting S") simp_all
+  have S: "toS S = toS (?M, ?N, ?U, ?k, ?D)"
+    unfolding S[symmetric] by simp
 
+  have
+    M: "M = map convert ?M" and
+    N: "N = mset (map mset ?N)" and
+    U: "U = mset (map mset ?U)"
+    using toSS[unfolded S] by auto
+
+  obtain D where
+    DCL: "mset D = C + {#L#}" and
+    D: "D \<in> set (?N @ ?U)"
+    using CL unfolding N U by auto
+  obtain C' L' where
+    setD: "set D = set (L' # C')" and
+    C': "mset C' = C" and
+    L: "L = L'"
+    using DCL by (metis ex_mset mset.simps(2) mset_eq_setD)
   have "find_first_unit_clause (?N @ ?U) ?M \<noteq> None"
-    apply (rule dist find_first_unit_clause_none[of C "?N @ ?U" ?M L, OF _])
-        using C dist apply auto[]
-       using C apply (cases S) apply (auto simp: raw_clauses_def)[1]
-      using MC apply auto[1]
-     using undef apply auto[1]
-    using L by auto
+    apply (rule dist find_first_unit_clause_none[of D "?N @ ?U" ?M L, OF _ D ])
+       using D assms(1) apply auto[1]
+      using MC setD DCL M MC unfolding C'[symmetric] apply auto[1]
+     using M undef apply auto[1]
+    unfolding setD L by auto
   then show False using prop_step S unfolding do_propagate_step_def by (cases S) auto
 qed
 
@@ -330,9 +295,8 @@ lemma find_conflict_None:
   by (induction Ns) auto
 
 lemma find_conflict_None_no_confl:
-  "find_conflict M (N@U) = None \<longleftrightarrow> no_step conflict_abs (M, N, U, k, None)"
-  by (auto simp add: find_conflict_None conflict_abs.simps raw_clauses_def cdcl\<^sub>W_mset_state_eq_eq
-    state_def)
+  "find_conflict M (N@U) = None \<longleftrightarrow> no_step conflict (toS (M, N, U, k, None))"
+  by (auto simp add: find_conflict_None conflict.simps)
 
 definition do_conflict_step where
 "do_conflict_step S =
@@ -344,43 +308,40 @@ definition do_conflict_step where
   | S \<Rightarrow> S)"
 
 lemma do_conflict_step:
-  "do_conflict_step S \<noteq> S \<Longrightarrow> conflict_abs S (do_conflict_step S)"
-  apply (cases S, cases "conc_conflicting S")
-  unfolding conflict_abs.simps do_conflict_step_def
-  by (auto dest!:find_conflict_Some split: option.splits simp: cdcl\<^sub>W_mset_state_eq_eq state_def
-    raw_clauses_def)
+  "do_conflict_step S \<noteq> S \<Longrightarrow> conflict (toS S) (toS (do_conflict_step S))"
+  apply (cases S, cases "raw_conflicting S")
+  unfolding conflict.simps do_conflict_step_def
+  by (auto dest!:find_conflict_Some split: option.splits)
 
 lemma do_conflict_step_no_step:
-  "do_conflict_step S = S \<Longrightarrow> no_step conflict_abs S"
-  apply (cases S, cases "conc_conflicting S")
+  "do_conflict_step S = S \<Longrightarrow> no_step conflict (toS S)"
+  apply (cases S, cases "raw_conflicting S")
   unfolding do_conflict_step_def
   using find_conflict_None_no_confl[of "raw_trail S" "raw_init_clss S" "raw_learned_clss S"
       "raw_backtrack_lvl S"]
-  by (auto split: option.split elim: conflict_absE)
+  by (auto split: option.splits elim!: conflictE)
 
 lemma do_conflict_step_option[simp]:
-  "conc_conflicting S \<noteq> None \<Longrightarrow> do_conflict_step S = S"
-  unfolding do_conflict_step_def by (cases S, cases "conc_conflicting S") auto
+  "raw_conflicting S \<noteq> None \<Longrightarrow> do_conflict_step S = S"
+  unfolding do_conflict_step_def by (cases S, cases "raw_conflicting S") auto
 
-lemma do_conflict_step_conflicting[dest]:
-  "do_conflict_step S \<noteq> S \<Longrightarrow> conc_conflicting (do_conflict_step S) \<noteq> None"
-  unfolding do_conflict_step_def by (cases S, cases "conc_conflicting S") (auto split: option.splits)
+lemma do_conflict_step_raw_conflicting[dest]:
+  "do_conflict_step S \<noteq> S \<Longrightarrow> raw_conflicting (do_conflict_step S) \<noteq> None"
+  unfolding do_conflict_step_def by (cases S, cases "raw_conflicting S") (auto split: option.splits)
 
-(* definition do_cp_step where
+definition do_cp_step where
 "do_cp_step S =
   (do_propagate_step o do_conflict_step) S"
 
 lemma cp_step_is_cdcl\<^sub>W_cp:
   assumes H: "do_cp_step S \<noteq> S"
-  shows "cdcl\<^sub>W_abs_cp S (do_cp_step S)"
+  shows "cdcl\<^sub>W_cp (toS S) (toS (do_cp_step S))"
 proof -
   show ?thesis
   proof (cases "do_conflict_step S \<noteq> S")
     case True
-    then have "do_propagate_step (do_conflict_step S) = do_conflict_step S"
-      by auto
     then show ?thesis
-      by (auto simp add: do_conflict_step do_conflict_step_conflicting do_cp_step_def True)
+      by (auto simp add: do_conflict_step do_conflict_step_raw_conflicting do_cp_step_def)
   next
     case False
     then have confl[simp]: "do_conflict_step S = S" by simp
@@ -391,11 +352,11 @@ proof -
         using H by (simp add: do_cp_step_def)
       next
         case False
-        let ?S = "S"
-        let ?T = "do_propagate_step S"
-        let ?U = "do_conflict_step (do_propagate_step S)"
-        have propa: "propagate S ?T" using False do_propgate_step by blast
-        moreover have ns: "no_step conflict S" using confl do_conflict_step_no_step by blast
+        let ?S = "toS S"
+        let ?T = "toS (do_propagate_step S)"
+        let ?U = "toS (do_conflict_step (do_propagate_step S))"
+        have propa: "propagate (toS S) ?T" using False do_propgate_step by blast
+        moreover have ns: "no_step conflict (toS S)" using confl do_conflict_step_no_step by blast
         ultimately show ?thesis
           using cdcl\<^sub>W_cp.intros(2)[of ?S ?T] confl unfolding do_cp_step_def by auto
       qed
@@ -412,37 +373,33 @@ lemma no_cdcl\<^sub>W_cp_iff_no_propagate_no_conflict:
   by (auto simp: cdcl\<^sub>W_cp.simps)
 
 lemma do_cp_step_eq_no_step:
-  assumes
-    H: "do_cp_step S = S" and "
-    \<forall>c \<in> set (raw_init_clss S @ raw_learned_clss S). distinct c"
-  shows "no_step cdcl\<^sub>W_cp S"
+  assumes H: "do_cp_step S = S" and "\<forall>c \<in> set (raw_init_clss S @ raw_learned_clss S). distinct c"
+  shows "no_step cdcl\<^sub>W_cp (toS S)"
   unfolding no_cdcl\<^sub>W_cp_iff_no_propagate_no_conflict
-  using assms apply (cases S, cases "conc_conflicting S")
+  using assms apply (cases S, cases "raw_conflicting S")
   using do_propagate_step_no_step[of S]
   by (auto dest!: do_cp_step_eq_no_prop_no_confl[simplified] do_conflict_step_no_step
     split: option.splits)
 
 lemma cdcl\<^sub>W_cp_cdcl\<^sub>W_st: "cdcl\<^sub>W_cp S S' \<Longrightarrow> cdcl\<^sub>W\<^sup>*\<^sup>* S S'"
   by (simp add: cdcl\<^sub>W_cp_tranclp_cdcl\<^sub>W tranclp_into_rtranclp)
-  
+
+lemma cdcl\<^sub>W_all_struct_inv_rough_state[simp]: "cdcl\<^sub>W_all_struct_inv (toS (rough_state_of S))"
+  using rough_state_of by auto
+
+lemma [simp]: "cdcl\<^sub>W_all_struct_inv (toS S) \<Longrightarrow> rough_state_of (state_of S) = S"
+  by (simp add: state_of_inverse)
+
 lemma rough_state_of_state_of_do_cp_step[simp]:
   "rough_state_of (state_of (do_cp_step (rough_state_of S))) = do_cp_step (rough_state_of S)"
 proof -
-  have "cdcl\<^sub>W_all_struct_inv (do_cp_step (rough_state_of S))"
+  have "cdcl\<^sub>W_all_struct_inv (toS (do_cp_step (rough_state_of S)))"
     apply (cases "do_cp_step (rough_state_of S) = (rough_state_of S)")
       apply simp
     using cp_step_is_cdcl\<^sub>W_cp[of "rough_state_of S"] cdcl\<^sub>W_all_struct_inv_rough_state[of S]
     cdcl\<^sub>W_cp_cdcl\<^sub>W_st rtranclp_cdcl\<^sub>W_all_struct_inv_inv by blast
   then show ?thesis by auto
 qed
- *)
-lemma cdcl\<^sub>W_all_struct_inv_rough_state[simp]:
-  "cdcl\<^sub>W_mset.cdcl\<^sub>W_all_struct_inv (state (rough_state_of S))"
-  using rough_state_of by auto
-
-lemma [simp]: "cdcl\<^sub>W_mset.cdcl\<^sub>W_all_struct_inv (state S) \<Longrightarrow> rough_state_of (state_of S) = S"
-  by (simp add: state_of_inverse)
-
 
 paragraph \<open>Skip\<close>
 fun do_skip_step :: "'v cdcl\<^sub>W_state_inv_st \<Rightarrow> 'v cdcl\<^sub>W_state_inv_st" where
@@ -453,41 +410,50 @@ fun do_skip_step :: "'v cdcl\<^sub>W_state_inv_st \<Rightarrow> 'v cdcl\<^sub>W_
 "do_skip_step S = S"
 
 lemma do_skip_step:
-  "do_skip_step S \<noteq> S \<Longrightarrow> skip_abs S (do_skip_step S)"
+  "do_skip_step S \<noteq> S \<Longrightarrow> skip (toS S) (toS (do_skip_step S))"
   apply (induction S rule: do_skip_step.induct)
-  by (auto simp add: skip_abs.simps)
+  by (auto simp add: skip.simps)
 
 lemma do_skip_step_no:
-  "do_skip_step S = S \<Longrightarrow> no_step skip_abs S"
+  "do_skip_step S = S \<Longrightarrow> no_step skip (toS S)"
   by (induction S rule: do_skip_step.induct)
-     (auto simp add: other split: if_split_asm elim!: skip_absE)
+     (auto simp add: other split: if_split_asm elim: skipE)
 
-lemma do_skip_step_trail_is_None[iff]:
+lemma do_skip_step_raw_trail_is_None[iff]:
   "do_skip_step S = (a, b, c, d, None) \<longleftrightarrow> S = (a, b, c, d, None)"
   by (cases S rule: do_skip_step.cases) auto
 
 paragraph \<open>Resolve\<close>
+fun maximum_level_code:: "'a literal list \<Rightarrow> ('a, 'a literal list) ann_lit list \<Rightarrow> nat"
+  where
+"maximum_level_code [] _ = 0" |
+"maximum_level_code (L # Ls) M = max (get_level M L) (maximum_level_code Ls M)"
+
+lemma maximum_level_code_eq_get_maximum_level[code, simp]:
+  "maximum_level_code D M = get_maximum_level M (mset D)"
+  by (induction D) (auto simp add: get_maximum_level_plus)
+
 fun do_resolve_step :: "'v cdcl\<^sub>W_state_inv_st \<Rightarrow> 'v cdcl\<^sub>W_state_inv_st" where
 "do_resolve_step (Propagated L C # Ls, N, U, k, Some D) =
-  (if -L \<in> set D \<and> get_maximum_level (Propagated L C # Ls) (mset (remove1 (-L) D)) = k
+  (if -L \<in> set D \<and> maximum_level_code (remove1 (-L) D) (Propagated L C # Ls) = k
   then (Ls, N, U, k, Some (remdups (remove1 L C @ remove1 (-L) D)))
   else (Propagated L C # Ls, N, U, k, Some D))" |
 "do_resolve_step S = S"
 
 lemma do_resolve_step:
-  "cdcl\<^sub>W_mset.cdcl\<^sub>W_all_struct_inv (state S) \<Longrightarrow> do_resolve_step S \<noteq> S
-  \<Longrightarrow> resolve_abs S (do_resolve_step S)"
+  "cdcl\<^sub>W_all_struct_inv (toS S) \<Longrightarrow> do_resolve_step S \<noteq> S
+  \<Longrightarrow> resolve (toS S) (toS (do_resolve_step S))"
 proof (induction S rule: do_resolve_step.induct)
   case (1 L C M N U k D)
   then have
-    LD: "- L \<in> set D" and
+    "- L \<in> set D" and
     M: "maximum_level_code (remove1 (-L) D) (Propagated L C # M) = k"
     by (cases "mset D - {#- L#} = {#}",
         auto dest!: get_maximum_level_exists_lit_of_max_level[of _ "Propagated L C # M"]
         split: if_split_asm)+
-  have "cdcl\<^sub>W_mset.every_mark_is_a_conflict (state (Propagated L C # M, N, U, k, Some D))"
-    using 1(1) unfolding cdcl\<^sub>W_mset.cdcl\<^sub>W_all_struct_inv_def cdcl\<^sub>W_mset.cdcl\<^sub>W_conflicting_def by fast
-  then have LC: "L \<in> set C" by fastforce
+  have "every_mark_is_a_conflict (toS (Propagated L C # M, N, U, k, Some D))"
+    using 1(1) unfolding cdcl\<^sub>W_all_struct_inv_def cdcl\<^sub>W_conflicting_def by fast
+  then have "L \<in> set C" by fastforce
   then obtain C' where C: "mset C = C' + {#L#}"
     by (metis add.commute in_multiset_in_set insert_DiffM)
   obtain D' where D: "mset D = D' + {#-L#}"
@@ -495,50 +461,60 @@ proof (induction S rule: do_resolve_step.induct)
   have D'L:  "D' + {#- L#} - {#-L#} = D'" by (auto simp add: multiset_eq_iff)
 
   have CL: "mset C - {#L#} + {#L#} = mset C" using \<open>L \<in> set C\<close> by (auto simp add: multiset_eq_iff)
-  have max: "get_maximum_level (Propagated L (C' + {#L#}) # map mmset_of_mlit' M) D' = k"
+  have "get_maximum_level (Propagated L (C' + {#L#}) # map convert M) D' = k"
     using M[simplified] unfolding maximum_level_code_eq_get_maximum_level C[symmetric] CL
-    by (metis D D'L get_maximum_level_map_convert list.simps(9) mmset_of_mlit'.simps(1))
-  have "distinct_mset (mset C)" and "distinct_mset (mset D)"
-    using \<open>cdcl\<^sub>W_mset.cdcl\<^sub>W_all_struct_inv (state (Propagated L C # M, N, U, k, Some D))\<close>
-    unfolding cdcl\<^sub>W_mset.cdcl\<^sub>W_all_struct_inv_def cdcl\<^sub>W_mset.distinct_cdcl\<^sub>W_state_def
-    by auto
-  then have conf: "(mset C - {#L#}) #\<union> (mset D - {#- L#}) =
-    remdups_mset (mset C - {#L#} + (mset D - {#- L#}))"
-    by (auto simp: distinct_mset_rempdups_union_mset)
-  show ?case
-    apply (rule resolve_abs_rule)
-    using LC LD max M conf C D by (auto simp: subset_mset.sup.commute cdcl\<^sub>W_mset_state_eq_eq
-      state_def)
+    by (metis D D'L convert.simps(1) get_maximum_level_map_convert list.simps(9))
+  then have
+    "resolve
+       (map convert (Propagated L C # M), mset `# mset N, mset `# mset U, k, Some (mset D))
+       (map convert M, mset `# mset N, mset `# mset U, k,
+         Some (((mset D - {#-L#}) #\<union> (mset C - {#L#}))))"
+    unfolding resolve.simps
+      by (simp add: C D)
+  moreover have
+    "(map convert (Propagated L C # M), mset `# mset N, mset `# mset U, k, Some (mset D))
+     = toS (Propagated L C # M, N, U, k, Some D)"
+    by (auto simp: mset_map)
+  moreover
+    have "distinct_mset (mset C)" and "distinct_mset (mset D)"
+      using \<open>cdcl\<^sub>W_all_struct_inv (toS (Propagated L C # M, N, U, k, Some D))\<close>
+      unfolding cdcl\<^sub>W_all_struct_inv_def distinct_cdcl\<^sub>W_state_def
+      by auto
+    then have "(mset C - {#L#}) #\<union> (mset D - {#- L#}) =
+      remdups_mset (mset C - {#L#} + (mset D - {#- L#}))"
+      by (auto simp: distinct_mset_rempdups_union_mset)
+    then have "(map convert M, mset `# mset N, mset `# mset U, k,
+    Some ((mset D - {#- L#}) #\<union> (mset C - {#L#})))
+    = toS (do_resolve_step (Propagated L C # M, N, U, k, Some D))"
+    using \<open>- L \<in> set D\<close> M by (auto simp:ac_simps mset_map)
+  ultimately show ?case
+    by simp
 qed auto
 
 lemma do_resolve_step_no:
-  "do_resolve_step S = S \<Longrightarrow> no_step resolve_abs S"
-  apply (cases S; cases "raw_trail S"; cases "raw_conflicting S")
+  "do_resolve_step S = S \<Longrightarrow> no_step resolve (toS S)"
+  apply (cases S; cases "hd (raw_trail S)";cases "raw_trail S"; cases "raw_conflicting S")
   by (auto
-    elim!: resolve_absE  split: if_split_asm
+    elim!: resolveE  split: if_split_asm
     dest!: union_single_eq_member
     simp del: in_multiset_in_set get_maximum_level_map_convert
-    simp: get_maximum_level_map_convert[symmetric] do_resolve_step)
+    simp: get_maximum_level_map_convert[symmetric])
 
-lemma rough_state_of_state_of_resolve[simp]:
-  "cdcl\<^sub>W_mset.cdcl\<^sub>W_all_struct_inv (state S) \<Longrightarrow> 
-    rough_state_of (state_of (do_resolve_step S)) = do_resolve_step S"
+lemma  rough_state_of_state_of_resolve[simp]:
+  "cdcl\<^sub>W_all_struct_inv (toS S) \<Longrightarrow> rough_state_of (state_of (do_resolve_step S)) = do_resolve_step S"
   apply (rule state_of_inverse)
   apply (cases "do_resolve_step S = S")
    apply simp
-  using do_resolve_step[of S]
-  by (auto simp add: resolve_resolve_abs[symmetric]
-    dest!: cdcl\<^sub>W_mset.other cdcl\<^sub>W_mset.resolve cdcl\<^sub>W_mset.bj
-    simp: cdcl\<^sub>W_mset.cdcl\<^sub>W_all_struct_inv_inv)
+  by (blast dest: other resolve bj do_resolve_step cdcl\<^sub>W_all_struct_inv_inv)
 
-lemma do_resolve_step_trail_is_None[iff]:
+lemma do_resolve_step_raw_trail_is_None[iff]:
   "do_resolve_step S = (a, b, c, d, None) \<longleftrightarrow> S = (a, b, c, d, None)"
   by (cases S rule: do_resolve_step.cases) auto
 
 paragraph \<open>Backjumping\<close>
 lemma get_all_ann_decomposition_map_convert:
-  "(get_all_ann_decomposition (map mmset_of_mlit' M)) =
-    map (\<lambda>(a, b). (map mmset_of_mlit' a, map mmset_of_mlit' b)) (get_all_ann_decomposition M)"
+  "(get_all_ann_decomposition (map convert M)) =
+    map (\<lambda>(a, b). (map convert a, map convert b)) (get_all_ann_decomposition M)"
   apply (induction M rule: ann_lit_list_induct)
     apply simp
   by (rename_tac L xs, case_tac "get_all_ann_decomposition xs"; auto)+
@@ -546,17 +522,18 @@ lemma get_all_ann_decomposition_map_convert:
 lemma do_backtrack_step:
   assumes
     db: "do_backtrack_step S \<noteq> S" and
-    inv: "cdcl\<^sub>W_mset.cdcl\<^sub>W_all_struct_inv (state S)"
-  shows "backtrack_abs S (do_backtrack_step S)"
+    inv: "cdcl\<^sub>W_all_struct_inv (toS S)"
+  shows "backtrack (toS S) (toS (do_backtrack_step S))"
   proof (cases S, cases "raw_conflicting S", goal_cases)
     case (1 M N U k E)
-    then show ?case using db by (auto)
+    then show ?case using db by auto
   next
     case (2 M N U k E C) note S = this(1) and confl = this(2)
     have E: "E = Some C" using S confl by auto
 
     obtain L j where fd: "find_level_decomp M C [] k = Some (L, j)"
-      using db unfolding S E  by (cases C) (auto split: if_split_asm option.splits)
+      using db unfolding S E  by (cases C) (auto split: if_split_asm option.splits list.splits 
+        ann_lit.splits)
     have
       "L \<in> set C" and
       j: "get_maximum_level M (mset (remove1 L C)) = j" and
@@ -564,48 +541,42 @@ lemma do_backtrack_step:
       using find_level_decomp_some[OF fd] by auto
     obtain C' where C: "mset C = mset C' + {#L#}"
       using \<open>L \<in> set C\<close> by (metis add.commute ex_mset in_multiset_in_set insert_DiffM)
-    obtain M\<^sub>2 where M\<^sub>2: "bt_cut j M = Some M\<^sub>2"
+    obtain M2 where M2: "bt_cut j M = Some M2"
       using db fd unfolding S E by (auto split: option.splits)
     have "no_dup M" and k: "k = count_decided (filter is_decided M)"
-      using inv S unfolding cdcl\<^sub>W_mset.cdcl\<^sub>W_all_struct_inv_def 
-      cdcl\<^sub>W_mset.cdcl\<^sub>W_M_level_inv_def by (auto simp: comp_def)
-    then obtain M1 K where M1: "M\<^sub>2 = Decided K # M1" and lev_K: "get_level M K = j + 1"
-      using bt_cut_some_decomp[OF _ M\<^sub>2] by (cases M\<^sub>2) auto
-    obtain c where c: "M = c @ Decided K # M1"
-       using bt_cut_in_get_all_ann_decomposition[OF \<open>no_dup M\<close> M\<^sub>2]
-       unfolding M1 by fastforce
-    have "j \<le> k" unfolding c j[symmetric] k
+      using inv unfolding cdcl\<^sub>W_all_struct_inv_def cdcl\<^sub>W_M_level_inv_def S by (auto simp: comp_def)
+    then obtain M1 K c where 
+      M1: "M2 = Decided K # M1" and lev_K: "get_level M K = j + 1" and
+      c: "M = c @ M2 "
+      using bt_cut_some_decomp[OF _ M2] by (cases M2) auto
+     have "j \<le> k" unfolding c j[symmetric] k
       by (metis (mono_tags, lifting) count_decided_ge_get_maximum_level filter_cong filter_filter)
     have max_l_j: "maximum_level_code C' M = j"
-      using db fd M\<^sub>2 C unfolding S E by (auto
+      using db fd M2 C unfolding S E by (auto
           split: option.splits list.splits ann_lit.splits
           dest!: find_level_decomp_some)[1]
     have "get_maximum_level M (mset C) \<ge> k"
       using \<open>L \<in> set C\<close> levL get_maximum_level_ge_get_level by (metis set_mset_mset)
     moreover have "get_maximum_level M (mset C) \<le> k"
       using get_maximum_level_exists_lit_of_max_level[of "mset C" M] inv
-        cdcl\<^sub>W_mset.cdcl\<^sub>W_M_level_inv_get_level_le_backtrack_lvl[of "state S"]
-      unfolding C cdcl\<^sub>W_mset.cdcl\<^sub>W_all_struct_inv_def S by (auto dest: sym[of "get_level _ _"])
+        cdcl\<^sub>W_M_level_inv_get_level_le_backtrack_lvl[of "toS S"]
+      unfolding C cdcl\<^sub>W_all_struct_inv_def S by (auto dest: sym[of "get_level _ _"])
     ultimately have "get_maximum_level M (mset C) = k" by auto
 
-    obtain M2 where M2: "(M\<^sub>2, M2) \<in> set (get_all_ann_decomposition M)"
-      using bt_cut_in_get_all_ann_decomposition[OF \<open>no_dup M\<close> M\<^sub>2] by metis
+    obtain M2' where M2': "(M2, M2') \<in> set (get_all_ann_decomposition M)"
+      using bt_cut_in_get_all_ann_decomposition[OF \<open>no_dup M\<close> M2] by metis
     have decomp:
-      "(Decided K # (map mmset_of_mlit' M1),
-      (map mmset_of_mlit' M2)) \<in>
-      set (get_all_ann_decomposition (map mmset_of_mlit' M))"
-      using imageI[of _ _ "\<lambda>(a, b). (map mmset_of_mlit' a, map mmset_of_mlit' b)", OF M2] j
-      unfolding S E M1 by (auto simp add: get_all_ann_decomposition_map_convert)
-    have red: "(reduce_trail_to (map mmset_of_mlit' M1)
-      (M, N, C # U, get_maximum_level M (remove1_mset L (mset C)), None))
-      = (M1, N, C # U, get_maximum_level M (remove1_mset L (mset C)), None)"
-     using  M2 M1 by auto
+      "(Decided K # (map convert M1),
+      (map convert M2')) \<in>
+      set (get_all_ann_decomposition (map convert M))"
+      using imageI[of _ _ "\<lambda>(a, b). (map convert a, map convert b)", OF M2'] j
+      unfolding S E M1 by (simp add: get_all_ann_decomposition_map_convert)
     show ?case
-      apply (rule backtrack_abs_rule)
-        using M\<^sub>2 fd confl \<open>L \<in> set C\<close> j decomp levL \<open>get_maximum_level M (mset C) = k\<close>
+      apply (rule backtrack_rule)
+        using M2 fd confl \<open>L \<in> set C\<close> j decomp levL \<open>get_maximum_level M (mset C) = k\<close>
         unfolding S E M1 apply (auto simp: mset_map)[6]
-      using M\<^sub>2 fd j red lev_K unfolding S E M1 cdcl\<^sub>W_mset_state_eq_eq
-      by (auto simp: comp_def)[2]
+      using M2' M2 fd j lev_K unfolding S E M1 CDCL_W_Implementation.state_eq_def
+      by (auto simp: comp_def ac_simps)[2]
 qed
 
 lemma map_eq_list_length:
@@ -613,51 +584,54 @@ lemma map_eq_list_length:
   by auto
 
 lemma map_mmset_of_mlit_eq_cons:
-  assumes "map mmset_of_mlit' M = a @ c"
+  assumes "map convert M = a @ c"
   obtains a' c' where
-     "M = a' @  c'" and
-     "a = map mmset_of_mlit' a'" and
-     "c = map mmset_of_mlit' c'"
+     "M = a' @ c'" and
+     "a = map convert a'" and
+     "c = map convert c'"
   using that[of "take (length a) M" "drop (length a) M"]
   assms by (metis append_eq_conv_conj append_take_drop_id drop_map take_map)
 
-abbreviation "cdcl\<^sub>W_all_struct_inv S \<equiv> cdcl\<^sub>W_mset.cdcl\<^sub>W_all_struct_inv (state S)"
-    
+lemma Decided_convert_iff:
+  "Decided K = convert za \<longleftrightarrow> za = Decided K"
+  by (cases za) auto
+  
 lemma do_backtrack_step_no:
   assumes
     db: "do_backtrack_step S = S" and
-    inv: "cdcl\<^sub>W_all_struct_inv S"
-  shows "no_step backtrack_abs S"
-proof (rule ccontr, cases S, cases "conc_conflicting S", goal_cases)
+    inv: "cdcl\<^sub>W_all_struct_inv (toS S)"
+  shows "no_step backtrack (toS S)"
+proof (rule ccontr, cases S, cases "raw_conflicting S", goal_cases)
   case 1
-  then show ?case using db by (auto split: option.splits elim: backtrack_absE)
+  then show ?case using db by (auto split: option.splits elim: backtrackE)
 next
   case (2 M N U k E C) note bt = this(1) and S = this(2) and confl = this(3)
   obtain K j M1 M2 L D where
     CE: "raw_conflicting S = Some D" and
     LD: "L \<in># mset D" and
-    decomp: "(Decided K # M1, M2) \<in> set (get_all_ann_decomposition (trail S))" and
+    decomp: "(Decided K # M1, M2) \<in> set (get_all_ann_decomposition (raw_trail S))" and
     levL: "get_level (raw_trail S) L = raw_backtrack_lvl S"  and
     k: "get_level (raw_trail S) L = get_maximum_level (raw_trail S) (mset D)" and
     j: "get_maximum_level (raw_trail S) (remove1_mset L (mset D)) \<equiv> j" and
-    lev_K: "get_level (trail S) K = Suc j"
+    lev_K: "get_level (raw_trail S) K = Suc j"
     using bt apply clarsimp
-    apply (elim backtrack_absE)
+    apply (elim backtrackE)
     apply (cases S)
-    by (auto simp add: get_all_ann_decomposition_map_convert)
-  obtain c where c: "trail S = c @ M2 @ Decided K # M1"
+    by (auto simp add: get_all_ann_decomposition_map_convert reduce_trail_to
+      Decided_convert_iff)
+  obtain c where c: "raw_trail S = c @ M2 @ Decided K # M1"
     using decomp by blast
-  have "k = count_decided (trail S)" and n_d: "no_dup M"
-    using inv S unfolding cdcl\<^sub>W_mset.cdcl\<^sub>W_all_struct_inv_def 
-    cdcl\<^sub>W_mset.cdcl\<^sub>W_M_level_inv_def by (auto simp: comp_def)
+  have "k = count_decided (raw_trail S)" and n_d: "no_dup M"
+    using inv S unfolding cdcl\<^sub>W_all_struct_inv_def cdcl\<^sub>W_M_level_inv_def 
+    by (auto simp: comp_def)
   then have "k > j"
-    using j count_decided_ge_get_maximum_level[of "trail S" "remove1_mset L (mset D)"]
-    count_decided_ge_get_level[of K "trail S"]
+    using j count_decided_ge_get_maximum_level[of "raw_trail S" "remove1_mset L (mset D)"]
+    count_decided_ge_get_level[of K "raw_trail S"]
     unfolding k lev_K
     unfolding c by (auto simp: get_all_ann_decomposition_map_convert simp del: count_decided_ge_get_level)
   have [simp]: "L \<in> set D"
     using LD by auto
-  have CD: "C = mset D"
+  have CD: "C =  D"
     using CE confl by auto
   obtain D' where
     E: "E = Some D" and
@@ -683,9 +657,10 @@ next
   then have j': "j' = j" using find_level_decomp_some[OF fd_some] j S DD' by auto
 
   obtain c' M1' where cM: "M = c' @ Decided K # M1'"
-    apply (rule map_mmset_of_mlit_eq_cons[of M "c @ M2" "Decided K # M1"])
+    apply (rule map_mmset_of_mlit_eq_cons[of M "map convert (c @ M2)"
+      "map convert (Decided K # M1)"])
       using c S apply simp
-    apply (rule map_mmset_of_mlit_eq_cons[of _ "[Decided K]" " M1"])
+    apply (rule map_mmset_of_mlit_eq_cons[of _ "map convert [Decided K]" "map convert M1"])
      apply auto[]
     apply (rename_tac a b' aa b, case_tac aa)
      apply auto[]
@@ -702,26 +677,24 @@ next
 qed
 
 lemma rough_state_of_state_of_backtrack[simp]:
-  assumes inv: "cdcl\<^sub>W_all_struct_inv S"
-  shows "rough_state_of (state_of (do_backtrack_step S)) = do_backtrack_step S"
+  assumes inv: "cdcl\<^sub>W_all_struct_inv (toS S)"
+  shows "rough_state_of (state_of (do_backtrack_step S))= do_backtrack_step S"
 proof (rule state_of_inverse)
-  consider
-    (step)"backtrack_abs S (do_backtrack_step S)" |
-    (eq)"do_backtrack_step S = S"
+  consider 
+    (step) "backtrack (toS S) (toS (do_backtrack_step S))" |
+     (0) "do_backtrack_step S = S"
     using do_backtrack_step inv by blast
-  then show "do_backtrack_step S \<in> {S. cdcl\<^sub>W_all_struct_inv S}"
-     proof cases
-       case eq
-       then show ?thesis using inv by simp
-     next
-       case step
-       then have "cdcl\<^sub>W_mset.backtrack (state S) (state (do_backtrack_step S))"
-         using inv by (auto simp: backtrack_backtrack_abs)
-       then show ?thesis
-         using inv by (auto simp: cdcl\<^sub>W_mset.cdcl\<^sub>W_all_struct_inv_inv
-           dest!: cdcl\<^sub>W_mset.cdcl\<^sub>W_o.bj cdcl\<^sub>W_mset.cdcl\<^sub>W_bj.backtrack cdcl\<^sub>W_mset.cdcl\<^sub>W.other)
-     qed
-qed
+  then show "do_backtrack_step S \<in> {S. cdcl\<^sub>W_all_struct_inv (toS S)}"
+    proof cases
+      case 0
+      thus ?thesis using inv by simp
+    next
+      case step
+      then show ?thesis
+        using inv
+        by (auto dest!:  cdcl\<^sub>W.other cdcl\<^sub>W_o.bj cdcl\<^sub>W_bj.backtrack intro: cdcl\<^sub>W_all_struct_inv_inv)
+    qed  
+qed      
 
 paragraph \<open>Decide\<close>
 fun do_decide_step where
@@ -732,38 +705,35 @@ fun do_decide_step where
 "do_decide_step S = S"
 
 lemma do_decide_step:
-  fixes S :: "'v cdcl\<^sub>W_state_inv_st"
-  assumes  "do_decide_step S \<noteq> S"
-  shows "decide_abs S (do_decide_step S)"
-  using assms
-  apply (cases S, cases "conc_conflicting S")
+  "do_decide_step S \<noteq> S \<Longrightarrow> decide (toS S) (toS (do_decide_step S))"
+  apply (cases S, cases "raw_conflicting S")
   defer
-  apply (auto split: option.splits simp add: decide_abs.simps Decided_Propagated_in_iff_in_lits_of_l
+  apply (auto split: option.splits simp add: decide.simps
           dest: find_first_unused_var_undefined find_first_unused_var_Some
-          intro:)[1]
+          intro: atms_of_atms_of_ms_mono)[1]
 proof -
-  fix a :: "('v, 'v literal list) ann_lits" and
-        b :: "'v literal list list" and  c :: "'v literal list list" and
-        d :: nat and e :: "'v literal list option"
+  fix a :: "('a, 'a literal list) ann_lit list" and
+        b :: "'a literal list list" and  c :: "'a literal list list" and
+        d :: nat and e :: "'a literal list option"
   {
-    fix a :: "('v, 'v literal list) ann_lits" and
-        b :: "'v literal list list" and  c :: "'v literal list list" and
-        d :: nat and x2 :: "'v literal" and m :: "'v literal list"
+    fix a :: "('a, 'a literal list) ann_lit list" and
+        b :: "'a literal list list" and  c :: "'a literal list list" and
+        d :: nat and x2 :: "'a literal" and m :: "'a literal list"
     assume a1: "m \<in> set b"
     assume "x2 \<in> set m"
     then have f2: "atm_of x2 \<in> atms_of (mset m)"
       by simp
-    have "\<And>f. (f m::'v clause) \<in> f ` set b"
+    have "\<And>f. (f m::'a literal multiset) \<in> f ` set b"
       using a1 by blast
-    then have "\<And>f. (atms_of (f m)::'v set) \<subseteq> atms_of_ms (f ` set b)"
-      by simp
-    then have "\<And>n f. (n::'v) \<in> atms_of_ms (f ` set b) \<or> n \<notin> atms_of (f m)"
+    then have "\<And>f. (atms_of (f m)::'a set) \<subseteq> atms_of_ms (f ` set b)"
+     using atms_of_atms_of_ms_mono by blast
+    then have "\<And>n f. (n::'a) \<in> atms_of_ms (f ` set b) \<or> n \<notin> atms_of (f m)"
       by (meson contra_subsetD)
     then have "atm_of x2 \<in> atms_of_ms (mset ` set b)"
       using f2 by blast
   } note H = this
   {
-    fix m :: "'v literal list" and x2
+    fix m :: "'a literal list" and x2
     have "m \<in> set b \<Longrightarrow> x2 \<in> set m \<Longrightarrow> x2 \<notin> lits_of_l a \<Longrightarrow> - x2 \<notin> lits_of_l a \<Longrightarrow>
       \<exists>aa\<in>set b. \<not> atm_of ` set aa \<subseteq> atm_of ` lits_of_l a"
       by (meson atm_of_in_atm_of_set_in_uminus contra_subsetD rev_image_eqI)
@@ -771,42 +741,36 @@ proof -
 
   assume  "do_decide_step S \<noteq> S" and
      "S = (a, b, c, d, e)" and
-     "conc_conflicting S = None"
-  then show "decide_abs S (do_decide_step S)"
-    using H H' by (auto split: option.splits simp: lits_of_def decide_abs.simps
-      Decided_Propagated_in_iff_in_lits_of_l cdcl\<^sub>W_mset_state_eq_eq state_def
-      dest!: find_first_unused_var_Some)
+     "raw_conflicting S = None"
+  then show "decide (toS S) (toS (do_decide_step S))"
+    using H H' by (auto split: option.splits simp: decide.simps defined_lit_map lits_of_def
+      image_image atm_of_eq_atm_of dest!: find_first_unused_var_Some)
 qed
 
-lemma mmset_of_mlit'_eq_Decided[iff]: "mmset_of_mlit' z = Decided x \<longleftrightarrow> z = Decided x"
-  by (cases z) auto
-
 lemma do_decide_step_no:
-  "do_decide_step S = S \<Longrightarrow> no_step decide_abs S"
-  apply (cases S, cases "conc_conflicting S")
-  (* TODO Tune proof *)
+  "do_decide_step S = S \<Longrightarrow> no_step decide (toS S)"
+  apply (cases S, cases "raw_conflicting S")
   apply (auto simp: atms_of_ms_mset_unfold  Decided_Propagated_in_iff_in_lits_of_l lits_of_def
       dest!: atm_of_in_atm_of_set_in_uminus
-      elim!: decide_absE
+      elim!: decideE
       split: option.splits)+
-using atm_of_eq_atm_of by blast
+  using atm_of_eq_atm_of by blast+
+
 
 lemma rough_state_of_state_of_do_decide_step[simp]:
-  "cdcl\<^sub>W_all_struct_inv S \<Longrightarrow> rough_state_of (state_of (do_decide_step S)) = do_decide_step S"
+  "cdcl\<^sub>W_all_struct_inv (toS S) \<Longrightarrow> rough_state_of (state_of (do_decide_step S)) = do_decide_step S"
 proof (subst state_of_inverse, goal_cases)
   case 1
   then show ?case
-   using do_decide_step[of S]
     by (cases "do_decide_step S = S")
-      (auto dest!: cdcl\<^sub>W_mset.decide cdcl\<^sub>W_mset.other simp: cdcl\<^sub>W_mset.cdcl\<^sub>W_all_struct_inv_inv
-        decide_decide_abs[symmetric])
+      (auto dest: do_decide_step decide other intro: cdcl\<^sub>W_all_struct_inv_inv)
 qed simp
 
 lemma rough_state_of_state_of_do_skip_step[simp]:
-  "cdcl\<^sub>W_all_struct_inv S \<Longrightarrow> rough_state_of (state_of (do_skip_step S)) = do_skip_step S"
+  "cdcl\<^sub>W_all_struct_inv (toS S) \<Longrightarrow> rough_state_of (state_of (do_skip_step S)) = do_skip_step S"
   apply (subst state_of_inverse, cases "do_skip_step S = S")
    apply simp
-  by (blast dest: cdcl\<^sub>W_mset.other cdcl\<^sub>W_mset.skip bj do_skip_step cdcl\<^sub>W_mset.cdcl\<^sub>W_all_struct_inv_inv)+
+  by (blast dest: other skip bj do_skip_step cdcl\<^sub>W_all_struct_inv_inv)+
 
 subsubsection \<open>Code generation\<close>
 paragraph \<open>Type definition\<close>
@@ -815,7 +779,8 @@ text \<open>There are two invariants: one while applying conflict and propagate 
 
 declare rough_state_of_inverse[simp add]
 definition Con where
-  "Con xs = state_of (if cdcl\<^sub>W_all_struct_inv xs then xs else ([], [], [], 0, None))"
+  "Con xs = state_of (if cdcl\<^sub>W_all_struct_inv (toS (fst xs, snd xs)) then xs
+  else ([], [], [], 0, None))"
 
 lemma [code abstype]:
  "Con (rough_state_of S) = S"
@@ -824,12 +789,13 @@ lemma [code abstype]:
 definition do_cp_step' where
 "do_cp_step' S = state_of (do_cp_step (rough_state_of S))"
 
-typedef 'v cdcl\<^sub>W_state_inv_from_init_state = "{S::'v cdcl\<^sub>W_state_inv_st. cdcl\<^sub>W_all_struct_inv S
-  \<and> cdcl\<^sub>W_stgy\<^sup>*\<^sup>* (raw_S0_cdcl\<^sub>W (raw_init_clss S)) S}"
+typedef 'v cdcl\<^sub>W_state_inv_from_init_state = 
+  "{S:: 'v cdcl\<^sub>W_state_inv_st. cdcl\<^sub>W_all_struct_inv (toS S)
+    \<and> cdcl\<^sub>W_stgy\<^sup>*\<^sup>* (S0_cdcl\<^sub>W (raw_init_clss (toS S))) (toS S)}"
   morphisms rough_state_from_init_state_of state_from_init_state_of
 proof
-  show "([],[], [], 0, None) \<in> {S. cdcl\<^sub>W_all_struct_inv S
-    \<and> cdcl\<^sub>W_stgy\<^sup>*\<^sup>* (raw_S0_cdcl\<^sub>W (raw_init_clss S)) S}"
+  show "([],[], [], 0, None) \<in> {S. cdcl\<^sub>W_all_struct_inv (toS S)
+    \<and> cdcl\<^sub>W_stgy\<^sup>*\<^sup>* (S0_cdcl\<^sub>W (raw_init_clss (toS S))) (toS S)}"
     by (auto simp add: cdcl\<^sub>W_all_struct_inv_def)
 qed
 
@@ -845,15 +811,15 @@ instance
 end
 
 definition ConI where
-  "ConI S = state_from_init_state_of (if cdcl\<^sub>W_all_struct_inv S
-    \<and> cdcl\<^sub>W_stgy\<^sup>*\<^sup>* (raw_S0_cdcl\<^sub>W (raw_init_clss S)) S then S else ([], [], [], 0, None))"
+  "ConI S = state_from_init_state_of (if cdcl\<^sub>W_all_struct_inv (toS (fst S, snd S))
+    \<and> cdcl\<^sub>W_stgy\<^sup>*\<^sup>* (S0_cdcl\<^sub>W (raw_init_clss (toS S))) (toS S) then S else ([], [], [], 0, None))"
 
 lemma [code abstype]:
   "ConI (rough_state_from_init_state_of S) = S"
   using rough_state_from_init_state_of[of S] unfolding ConI_def
   by (simp add: rough_state_from_init_state_of_inverse)
 
-definition id_of_I_to :: "'v cdcl\<^sub>W_state_inv_from_init_state \<Rightarrow> 'v cdcl\<^sub>W_state_inv" where
+definition id_of_I_to:: "'v cdcl\<^sub>W_state_inv_from_init_state \<Rightarrow> 'v cdcl\<^sub>W_state_inv" where
 "id_of_I_to S = state_of (rough_state_from_init_state_of S)"
 
 lemma [code abstract]:
@@ -868,10 +834,10 @@ function do_full1_cp_step :: "'v cdcl\<^sub>W_state_inv \<Rightarrow> 'v cdcl\<^
 by auto
 termination
 proof (relation "{(T', T). (rough_state_of T', rough_state_of T) \<in> {(S', S).
-  (S', S) \<in> {(S', S). cdcl\<^sub>W_all_struct_inv S \<and> cdcl\<^sub>W_cp S S'}}}", goal_cases)
+  (toS S', toS S) \<in> {(S', S). cdcl\<^sub>W_all_struct_inv S \<and> cdcl\<^sub>W_cp S S'}}}", goal_cases)
   case 1
   show ?case
-    using wf_if_measure_f[OF wf_if_measure_f[OF cdcl\<^sub>W_cp_wf_all_inv, of ], of rough_state_of] .
+    using wf_if_measure_f[OF wf_if_measure_f[OF cdcl\<^sub>W_cp_wf_all_inv, of "toS"], of rough_state_of] .
 next
   case (2 S' S)
   then show ?case
@@ -881,9 +847,9 @@ next
 qed
 
 lemma do_full1_cp_step_fix_point_of_do_full1_cp_step:
-  "do_cp_step(rough_state_of (do_full1_cp_step S)) = rough_state_of (do_full1_cp_step S)"
+  "do_cp_step(rough_state_of (do_full1_cp_step S)) = (rough_state_of (do_full1_cp_step S))"
   by (rule do_full1_cp_step.induct[of "\<lambda>S. do_cp_step(rough_state_of (do_full1_cp_step S))
-       = rough_state_of (do_full1_cp_step S)"])
+       = (rough_state_of (do_full1_cp_step S))"])
     (metis (full_types) do_full1_cp_step.elims rough_state_of_state_of_do_cp_step do_cp_step'_def)
 
 lemma in_clauses_rough_state_of_is_distinct:
@@ -893,41 +859,41 @@ lemma in_clauses_rough_state_of_is_distinct:
     distinct_cdcl\<^sub>W_state_def)
 
 lemma do_full1_cp_step_full:
-  "full cdcl\<^sub>W_cp (rough_state_of S)
-    (rough_state_of (do_full1_cp_step S))"
+  "full cdcl\<^sub>W_cp (toS (rough_state_of S))
+    (toS (rough_state_of (do_full1_cp_step S)))"
   unfolding full_def
 proof (rule conjI, induction S rule: do_full1_cp_step.induct)
   case (1 S)
   then have f1:
-      "cdcl\<^sub>W_cp\<^sup>*\<^sup>* ((do_cp_step (rough_state_of S))) (
-         (rough_state_of (do_full1_cp_step (state_of (do_cp_step (rough_state_of S))))))
+      "cdcl\<^sub>W_cp\<^sup>*\<^sup>* (toS (do_cp_step (rough_state_of S))) (
+        toS (rough_state_of (do_full1_cp_step (state_of (do_cp_step (rough_state_of S))))))
       \<or> state_of (do_cp_step (rough_state_of S)) = S"
-    using rough_state_of_state_of_do_cp_step[of S] unfolding do_cp_step'_def by fastforce
+    using rough_state_of_state_of_do_cp_step unfolding do_cp_step'_def by fastforce
   have f2: "\<And>c. (if c = state_of (do_cp_step (rough_state_of c))
        then c else do_full1_cp_step (state_of (do_cp_step (rough_state_of c))))
      = do_full1_cp_step c"
     by (metis (full_types) do_cp_step'_def do_full1_cp_step.simps)
-  have f3: "\<not> cdcl\<^sub>W_cp  (rough_state_of S) (do_cp_step (rough_state_of S))
+  have f3: "\<not> cdcl\<^sub>W_cp (toS (rough_state_of S)) (toS (do_cp_step (rough_state_of S)))
     \<or> state_of (do_cp_step (rough_state_of S)) = S
-    \<or> cdcl\<^sub>W_cp\<^sup>+\<^sup>+ (rough_state_of S)
-        (rough_state_of (do_full1_cp_step (state_of (do_cp_step (rough_state_of S)))))"
+    \<or> cdcl\<^sub>W_cp\<^sup>+\<^sup>+ (toS (rough_state_of S))
+        (toS (rough_state_of (do_full1_cp_step (state_of (do_cp_step (rough_state_of S))))))"
     using f1 by (meson rtranclp_into_tranclp2)
   { assume "do_full1_cp_step S \<noteq> S"
     then have "do_cp_step (rough_state_of S) = rough_state_of S
-        \<longrightarrow> cdcl\<^sub>W_cp\<^sup>*\<^sup>* (rough_state_of S) (rough_state_of (do_full1_cp_step S))
+        \<longrightarrow> cdcl\<^sub>W_cp\<^sup>*\<^sup>* (toS (rough_state_of S)) (toS (rough_state_of (do_full1_cp_step S)))
       \<or> do_cp_step (rough_state_of S) \<noteq> rough_state_of S
         \<and> state_of (do_cp_step (rough_state_of S)) \<noteq> S"
       using f2 f1 by (metis (no_types))
     then have "do_cp_step (rough_state_of S) \<noteq> rough_state_of S
         \<and> state_of (do_cp_step (rough_state_of S)) \<noteq> S
-      \<or> cdcl\<^sub>W_cp\<^sup>*\<^sup>* (rough_state_of S) (rough_state_of (do_full1_cp_step S))"
+      \<or> cdcl\<^sub>W_cp\<^sup>*\<^sup>* (toS (rough_state_of S)) (toS (rough_state_of (do_full1_cp_step S)))"
       by (metis rough_state_of_state_of_do_cp_step)
-    then have "cdcl\<^sub>W_cp\<^sup>*\<^sup>* (rough_state_of S) (rough_state_of (do_full1_cp_step S))"
+    then have "cdcl\<^sub>W_cp\<^sup>*\<^sup>* (toS (rough_state_of S)) (toS (rough_state_of (do_full1_cp_step S)))"
       using f3 f2 by (metis (no_types) cp_step_is_cdcl\<^sub>W_cp tranclp_into_rtranclp) }
   then show ?case
     by fastforce
 next
-  show "no_step cdcl\<^sub>W_cp (rough_state_of (do_full1_cp_step S))"
+  show "no_step cdcl\<^sub>W_cp (toS (rough_state_of (do_full1_cp_step S)))"
     apply (rule do_cp_step_eq_no_step[OF do_full1_cp_step_fix_point_of_do_full1_cp_step[of S]])
     using in_clauses_rough_state_of_is_distinct unfolding do_cp_step'_def by blast
 qed
@@ -950,18 +916,18 @@ fun do_other_step where
        if V \<noteq> U then V else do_decide_step V)))"
 
 lemma do_other_step:
-  assumes inv: "cdcl\<^sub>W_all_struct_inv S" and
+  assumes inv: "cdcl\<^sub>W_all_struct_inv (toS S)" and
   st: "do_other_step S \<noteq> S"
-  shows "cdcl\<^sub>W_o S (do_other_step S)"
+  shows "cdcl\<^sub>W_o (toS S) (toS (do_other_step S))"
   using st inv by (auto split: if_split_asm
     simp add: Let_def
-    intro: do_skip_step do_resolve_step do_backtrack_step do_decide_step
-     cdcl\<^sub>W_o.intros cdcl\<^sub>W_bj.intros)
+    dest!: do_skip_step do_resolve_step do_backtrack_step do_decide_step
+    dest!: cdcl\<^sub>W_o.intros cdcl\<^sub>W_bj.intros)
 
 lemma do_other_step_no:
-  assumes inv: "cdcl\<^sub>W_all_struct_inv S" and
+  assumes inv: "cdcl\<^sub>W_all_struct_inv (toS S)" and
   st: "do_other_step S = S"
-  shows "no_step cdcl\<^sub>W_o S"
+  shows "no_step cdcl\<^sub>W_o (toS S)"
   using st inv by (auto split: if_split_asm elim: cdcl\<^sub>W_bjE
     simp add: Let_def cdcl\<^sub>W_bj.simps elim!: cdcl\<^sub>W_o.cases
     dest!: do_skip_step_no do_resolve_step_no do_backtrack_step_no do_decide_step_no)
@@ -973,9 +939,9 @@ proof (cases "do_other_step (rough_state_of S) = rough_state_of S")
   then show ?thesis by simp
 next
   case False
-  have "cdcl\<^sub>W_o (rough_state_of S) (do_other_step (rough_state_of S))"
+  have "cdcl\<^sub>W_o (toS (rough_state_of S)) (toS (do_other_step (rough_state_of S)))"
     by (metis False cdcl\<^sub>W_all_struct_inv_rough_state do_other_step["of" "rough_state_of S"])
-  then have "cdcl\<^sub>W_all_struct_inv (do_other_step (rough_state_of S))"
+  then have "cdcl\<^sub>W_all_struct_inv (toS (do_other_step (rough_state_of S)))"
     using cdcl\<^sub>W_all_struct_inv_inv cdcl\<^sub>W_all_struct_inv_rough_state other by blast
   then show ?thesis
     by (simp add: CollectI state_of_inverse)
@@ -1005,13 +971,14 @@ definition do_cdcl\<^sub>W_stgy_step' where
 "do_cdcl\<^sub>W_stgy_step' S = state_from_init_state_of (rough_state_of (do_cdcl\<^sub>W_stgy_step (id_of_I_to S)))"
 
 lemma toS_do_full1_cp_step_not_eq: "do_full1_cp_step S \<noteq> S \<Longrightarrow>
-    rough_state_of S \<noteq> rough_state_of (do_full1_cp_step S)"
+    toS (rough_state_of S) \<noteq> toS (rough_state_of (do_full1_cp_step S))"
 proof -
   assume a1: "do_full1_cp_step S \<noteq> S"
   then have "S \<noteq> do_cp_step' S"
     by fastforce
   then show ?thesis
-    by (metis (no_types) do_cp_step'_def  do_full1_cp_step_fix_point_of_do_full1_cp_step
+    by (metis (no_types) cp_step_is_cdcl\<^sub>W_cp do_cp_step'_def do_cp_step_eq_no_step
+      do_full1_cp_step_fix_point_of_do_full1_cp_step in_clauses_rough_state_of_is_distinct
       rough_state_of_inverse)
 qed
 
@@ -1021,7 +988,7 @@ declare do_full1_cp_step.simps[simp del]
 paragraph \<open>Correction of the transformation\<close>
 lemma do_cdcl\<^sub>W_stgy_step:
   assumes "do_cdcl\<^sub>W_stgy_step S \<noteq> S"
-  shows "cdcl\<^sub>W_stgy (rough_state_of S) (rough_state_of (do_cdcl\<^sub>W_stgy_step S))"
+  shows "cdcl\<^sub>W_stgy (toS (rough_state_of S)) (toS (rough_state_of (do_cdcl\<^sub>W_stgy_step S)))"
 proof (cases "do_full1_cp_step S = S")
   case False
   then show ?thesis
@@ -1029,46 +996,56 @@ proof (cases "do_full1_cp_step S = S")
     by (auto intro!: cdcl\<^sub>W_stgy.intros dest: toS_do_full1_cp_step_not_eq)
 next
   case True
-  have "cdcl\<^sub>W_o (rough_state_of S) (rough_state_of (do_other_step' S))"
+  have "cdcl\<^sub>W_o (toS (rough_state_of S)) (toS (rough_state_of (do_other_step' S)))"
     by (smt True assms cdcl\<^sub>W_all_struct_inv_rough_state do_cdcl\<^sub>W_stgy_step_def do_other_step
       rough_state_of_do_other_step' rough_state_of_inverse)
   moreover
     have
-      np: "no_step propagate (rough_state_of S)" and
-      nc: "no_step conflict (rough_state_of S)"
-        apply (metis True cdcl\<^sub>W_cp.simps do_cp_step_eq_no_step
-          do_full1_cp_step_fix_point_of_do_full1_cp_step in_clauses_rough_state_of_is_distinct)
+      np: "no_step propagate (toS (rough_state_of S))" and
+      nc: "no_step conflict (toS (rough_state_of S))"
+        apply (metis True do_cp_step_eq_no_prop_no_confl
+          do_full1_cp_step_fix_point_of_do_full1_cp_step do_propagate_step_no_step
+          in_clauses_rough_state_of_is_distinct)
       by (metis True do_conflict_step_no_step do_cp_step_eq_no_prop_no_confl
         do_full1_cp_step_fix_point_of_do_full1_cp_step)
-    then have "no_step cdcl\<^sub>W_cp (rough_state_of S)"
+    then have "no_step cdcl\<^sub>W_cp (toS (rough_state_of S))"
       by (simp add: cdcl\<^sub>W_cp.simps)
-  moreover have "full cdcl\<^sub>W_cp (rough_state_of (do_other_step' S))
-    (rough_state_of (do_full1_cp_step (do_other_step' S)))"
+  moreover have "full cdcl\<^sub>W_cp (toS (rough_state_of (do_other_step' S)))
+    (toS (rough_state_of (do_full1_cp_step (do_other_step' S))))"
     using do_full1_cp_step_full by auto
   ultimately show ?thesis
     using assms True unfolding do_cdcl\<^sub>W_stgy_step_def
     by (auto intro!: cdcl\<^sub>W_stgy.other' dest: toS_do_full1_cp_step_not_eq)
 qed
 
-lemma do_skip_step_trail_changed_or_conflict:
+lemma length_raw_trail_toS[simp]:
+  "length (raw_trail (toS S)) = length (raw_trail S)"
+  by (cases S) auto
+
+lemma raw_conflicting_noTrue_iff_toS[simp]:
+  "raw_conflicting (toS S) \<noteq> None \<longleftrightarrow> raw_conflicting S \<noteq> None"
+  by (cases S) auto
+
+lemma raw_trail_toS_neq_imp_raw_trail_neq:
+  "raw_trail (toS S) \<noteq> raw_trail (toS S') \<Longrightarrow> raw_trail S \<noteq> raw_trail S'"
+  by (cases S, cases S') auto
+
+lemma do_skip_step_raw_trail_changed_or_conflict:
   assumes d: "do_other_step S \<noteq> S"
-  and inv: "cdcl\<^sub>W_all_struct_inv S"
-  shows "trail S \<noteq> trail (do_other_step S)"
+  and inv: "cdcl\<^sub>W_all_struct_inv (toS S)"
+  shows "raw_trail S \<noteq> raw_trail (do_other_step S)"
 proof -
   have M: "\<And>M K M1 c. M = c @ K # M1 \<Longrightarrow> Suc (length M1) \<le> length M"
     by auto
-  have "cdcl\<^sub>W_M_level_inv S"
+  have "cdcl\<^sub>W_M_level_inv (toS S)"
     using inv unfolding cdcl\<^sub>W_all_struct_inv_def by auto
-  have "cdcl\<^sub>W_o S (do_other_step S)" using do_other_step[OF inv d] .
+  have "cdcl\<^sub>W_o (toS S) (toS (do_other_step S))" using do_other_step[OF inv d] .
   then show ?thesis
-    using \<open>cdcl\<^sub>W_M_level_inv S\<close>
-    proof (induction "do_other_step S" rule: cdcl\<^sub>W_o_induct_lev2)
+    using \<open>cdcl\<^sub>W_M_level_inv (toS S)\<close>
+    proof (induction "toS (do_other_step S)" rule: cdcl\<^sub>W_o_induct)
       case decide
       then show ?thesis
-        apply (cases S) (* TODO Tune proof *)
-        apply (auto dest!: find_first_unused_var_Some
-          simp: split: option.splits)
-        by (meson atm_of_in_atm_of_set_iff_in_set_or_uminus_in_set contra_subsetD)
+        by (auto simp add: raw_trail_toS_neq_imp_raw_trail_neq)[]
     next
     case (skip)
     then show ?case
@@ -1078,12 +1055,39 @@ proof -
       then show ?case
          by (cases S, cases "do_other_step S") force
     next
-      case (backtrack K i M1 M2 L D) note decomp = this(1) and confl_S = this(3) and undef = this(8)
-        and U = this(9)
+      case (backtrack L D K i M1 M2) note decomp = this(3) and confl_S = this(1) and i = this(6)
+        and U = this(8)
+      have H:"length M1 \<le> length (raw_trail (toS S))"
+        using decomp by (metis (mono_tags, lifting) in_get_all_ann_decomposition_trail_update_trail 
+          le_0_eq list.size(3) nat_le_linear trail_reduce_trail_to_drop)
+      have [simp]: "raw_cons_trail (Propagated L D)
+        (reduce_trail_to M1
+          (raw_add_learned_clss D
+            (raw_update_backtrack_lvl i
+              (raw_update_conflicting None (toS S)))))
+        =
+        (Propagated L D # M1,mset (map mset (raw_init_clss S)),
+          {#D#} + mset (map mset (raw_learned_clss S)),
+          i, None)"
+        apply (subst state_conv[of "raw_cons_trail _ _"])
+        using decomp H apply (cases S) apply (auto simp: reduce_trail_to 
+          dest!: )(* TODO tune proof *)
+       by (smt in_get_all_ann_decomposition_trail_update_trail length_raw_trail_toS raw_trail_conv 
+         toS.simps trail_reduce_trail_to_drop)
       then show ?case
+        using H
         apply (cases "do_other_step S")
-        apply (cases S)
-        by (auto split: if_split_asm simp: Let_def)
+        apply (auto split: if_split_asm simp: Let_def)
+            apply (cases S rule: do_skip_step.cases; auto split: if_split_asm)
+           apply (cases S rule: do_skip_step.cases; auto split: if_split_asm)
+
+          apply (cases S rule: do_backtrack_step.cases;
+            auto split: if_split_asm option.splits list.splits ann_lit.splits
+              dest!: bt_cut_some_decomp simp: Let_def)
+        using d U backtrack(4) apply (cases S rule: do_decide_step.cases; auto split: option.splits simp:
+            ac_simps reduce_trail_to comp_def)
+        
+        sorry
     qed
 qed
 
@@ -1091,60 +1095,59 @@ lemma do_full1_cp_step_induct:
   "(\<And>S. (S \<noteq>  do_cp_step' S \<Longrightarrow> P (do_cp_step' S)) \<Longrightarrow> P S) \<Longrightarrow> P a0"
   using do_full1_cp_step.induct by metis
 
-lemma do_cp_step_neq_trail_increase:
-  "\<exists>c. raw_trail (do_cp_step S) = c @ raw_trail S \<and>(\<forall>m \<in> set c. \<not> is_decided m)"
+lemma do_cp_step_neq_raw_trail_increase:
+  "\<exists>c. raw_trail (do_cp_step S) = c @ raw_trail  S \<and>(\<forall>m \<in> set c. \<not> is_decided m)"
   by (cases S, cases "raw_conflicting S")
      (auto simp add: do_cp_step_def do_conflict_step_def do_propagate_step_def split: option.splits)
 
-lemma do_full1_cp_step_neq_trail_increase:
+lemma do_full1_cp_step_neq_raw_trail_increase:
   "\<exists>c. raw_trail (rough_state_of (do_full1_cp_step S)) = c @ raw_trail (rough_state_of S)
     \<and> (\<forall>m \<in> set c. \<not> is_decided m)"
   apply (induction rule: do_full1_cp_step_induct)
   apply (rename_tac S, case_tac "do_cp_step' S = S")
     apply (simp add: do_full1_cp_step.simps)
-  by (smt Un_iff append_assoc do_cp_step'_def do_cp_step_neq_trail_increase do_full1_cp_step.simps
+  by (smt Un_iff append_assoc do_cp_step'_def do_cp_step_neq_raw_trail_increase do_full1_cp_step.simps
     rough_state_of_state_of_do_cp_step set_append)
 
-lemma do_cp_step_conflicting:
-  "conc_conflicting (rough_state_of S) \<noteq> None \<Longrightarrow> do_cp_step' S = S"
+lemma do_cp_step_raw_conflicting:
+  "raw_conflicting (rough_state_of S) \<noteq> None \<Longrightarrow> do_cp_step' S = S"
   unfolding do_cp_step'_def do_cp_step_def by simp
 
-lemma do_full1_cp_step_conflicting:
-  "conc_conflicting (rough_state_of S) \<noteq> None \<Longrightarrow> do_full1_cp_step S = S"
+lemma do_full1_cp_step_raw_conflicting:
+  "raw_conflicting (rough_state_of S) \<noteq> None \<Longrightarrow> do_full1_cp_step S = S"
   unfolding do_cp_step'_def do_cp_step_def
   apply (induction rule: do_full1_cp_step_induct)
   by (rename_tac S, case_tac "S \<noteq> do_cp_step' S")
-   (auto simp add: do_full1_cp_step.simps do_cp_step_conflicting)
+   (auto simp add: do_full1_cp_step.simps do_cp_step_raw_conflicting)
 
-lemma do_decide_step_not_conflicting_one_more_decide:
+lemma do_decide_step_not_raw_conflicting_one_more_decide:
   assumes
-    "conc_conflicting S = None" and
+    "raw_conflicting S = None" and
     "do_decide_step S \<noteq> S"
   shows "Suc (length (filter is_decided (raw_trail S)))
     = length (filter is_decided (raw_trail (do_decide_step S)))"
   using assms unfolding do_other_step'_def
-  by (cases S) (force simp: Let_def split: if_split_asm option.splits
+  by (cases S) (auto simp: Let_def split: if_split_asm option.splits
      dest!: find_first_unused_var_Some_not_all_incl)
 
-lemma do_decide_step_not_conflicting_one_more_decide_bt:
-  assumes "conc_conflicting S \<noteq> None" and
+lemma do_decide_step_not_raw_conflicting_one_more_decide_bt:
+  assumes "raw_conflicting S \<noteq> None" and
   "do_decide_step S \<noteq> S"
-  shows "length (filter is_decided (raw_trail S)) <
-    length (filter is_decided (raw_trail (do_decide_step S)))"
-  using assms unfolding do_other_step'_def by (cases S, cases "conc_conflicting S")
+  shows "length (filter is_decided (raw_trail S)) < length (filter is_decided (raw_trail (do_decide_step S)))"
+  using assms unfolding do_other_step'_def by (cases S, cases "raw_conflicting S")
     (auto simp add: Let_def split: if_split_asm option.splits)
 
-lemma do_other_step_not_conflicting_one_more_decide_bt:
+lemma do_other_step_not_raw_conflicting_one_more_decide_bt:
   assumes
-    "conc_conflicting (rough_state_of S) \<noteq> None" and
-    "conc_conflicting (rough_state_of (do_other_step' S)) = None" and
+    "raw_conflicting (rough_state_of S) \<noteq> None" and
+    "raw_conflicting (rough_state_of (do_other_step' S)) = None" and
     "do_other_step' S \<noteq> S"
   shows "length (filter is_decided (raw_trail (rough_state_of S)))
     > length (filter is_decided (raw_trail (rough_state_of (do_other_step' S))))"
 proof (cases S, goal_cases)
   case (1 y) note S = this(1) and inv = this(2)
   obtain M N U k E where y: "y = (M, N, U, k, Some E)"
-    using assms(1) S inv by (cases y, cases "conc_conflicting y") auto
+    using assms(1) S inv by (cases y, cases "raw_conflicting y") auto
   have M: "rough_state_of (state_of (M, N, U, k,  Some E)) = (M, N, U, k,  Some E)"
     using inv y by (auto simp add: state_of_inverse)
   have bt: "do_other_step' S = state_of (do_backtrack_step (rough_state_of S))"
@@ -1165,30 +1168,25 @@ proof (cases S, goal_cases)
                (do_skip_step (rough_state_of c)))))
         = rough_state_of (do_other_step' c)"
         by (simp add: rough_state_of_do_other_step')
-      have "
-        (raw_trail (rough_state_of (do_other_step' S)),
-        raw_init_clss (rough_state_of (do_other_step' S)),
+      have "(raw_trail (rough_state_of (do_other_step' S)), raw_init_clss (rough_state_of (do_other_step' S)),
           raw_learned_clss (rough_state_of (do_other_step' S)),
           raw_backtrack_lvl (rough_state_of (do_other_step' S)), None)
         = rough_state_of (do_other_step' S)"
-        using assms(2) by (cases "do_other_step' S") auto
+        using assms(2) by (metis (no_types) state_conv)
       then show ?thesis
-        using f3 2 by (metis (no_types) do_decide_step.simps(2) do_resolve_step_trail_is_None
-          do_skip_step_trail_is_None rough_state_of_inverse)
+        using f3 2 by (metis (no_types) do_decide_step.simps(2) do_resolve_step_raw_trail_is_None
+          do_skip_step_raw_trail_is_None rough_state_of_inverse)
     qed
-  have "no_dup (trail (rough_state_of S))"
-    using rough_state_of[of S] unfolding cdcl\<^sub>W_all_struct_inv_def cdcl\<^sub>W_M_level_inv_def
-    by (cases S) (auto simp: comp_def)
-  then show ?case
+  show ?case
     using assms(2) S unfolding bt y inv
     apply simp
-    by (auto simp add: M bt_cut_not_none comp_def
-      split: option.splits
-      dest: bt_cut_some_decomp)
+    by (auto simp add: M bt_cut_not_none
+          split: option.splits ann_lit.splits list.splits
+          dest!: bt_cut_some_decomp)
 qed
 
-lemma do_other_step_not_conflicting_one_more_decide:
-  assumes "conc_conflicting (rough_state_of S) = None" and
+lemma do_other_step_not_raw_conflicting_one_more_decide:
+  assumes "raw_conflicting (rough_state_of S) = None" and
   "do_other_step' S \<noteq> S"
   shows "1 + length (filter is_decided (raw_trail (rough_state_of S)))
     = length (filter is_decided (raw_trail (rough_state_of (do_other_step' S))))"
@@ -1208,7 +1206,7 @@ proof (cases S, goal_cases)
   have "do_other_step (rough_state_of S) \<noteq> rough_state_of S"
     using assms(2) unfolding S M y do_other_step'_def by (metis (no_types))
   then show ?case
-    using f6 f5 f4 by (simp add: assms(1) do_decide_step_not_conflicting_one_more_decide
+    using f6 f5 f4 by (simp add: assms(1) do_decide_step_not_raw_conflicting_one_more_decide
       do_other_step'_def)
 qed
 
@@ -1216,89 +1214,71 @@ lemma rough_state_of_state_of_do_skip_step_rough_state_of[simp]:
   "rough_state_of (state_of (do_skip_step (rough_state_of S))) = do_skip_step (rough_state_of S)"
   by (smt do_other_step.simps rough_state_of_inverse rough_state_of_state_of_do_other_step)
 
-lemma conflicting_do_resolve_step_iff[iff]:
-  "conc_conflicting (do_resolve_step S) = None \<longleftrightarrow> conflicting S = None"
+lemma raw_conflicting_do_resolve_step_iff[iff]:
+  "raw_conflicting (do_resolve_step S) = None \<longleftrightarrow> raw_conflicting S = None"
   by (cases S rule: do_resolve_step.cases)
    (auto simp add: Let_def split: option.splits)
 
-lemma conflicting_do_skip_step_iff[iff]:
-  "conc_conflicting (do_skip_step S) = None \<longleftrightarrow> conflicting S = None"
+lemma raw_conflicting_do_skip_step_iff[iff]:
+  "raw_conflicting (do_skip_step S) = None \<longleftrightarrow> raw_conflicting S = None"
   by (cases S rule: do_skip_step.cases)
      (auto simp add: Let_def split: option.splits)
 
-lemma conflicting_do_decide_step_iff[iff]:
-  "conc_conflicting (do_decide_step S) = None \<longleftrightarrow> conflicting S = None"
+lemma raw_conflicting_do_decide_step_iff[iff]:
+  "raw_conflicting (do_decide_step S) = None \<longleftrightarrow> raw_conflicting S = None"
   by (cases S rule: do_decide_step.cases)
      (auto simp add: Let_def split: option.splits)
 
-lemma conflicting_do_backtrack_step_imp[simp]:
-  "do_backtrack_step S \<noteq> S \<Longrightarrow> conflicting (do_backtrack_step S) = None"
+lemma raw_conflicting_do_backtrack_step_imp[simp]:
+  "do_backtrack_step S \<noteq> S \<Longrightarrow> raw_conflicting (do_backtrack_step S) = None"
   by (cases S rule: do_backtrack_step.cases)
      (auto simp add: Let_def split: list.splits option.splits ann_lit.splits)
 
-lemma do_skip_step_eq_iff_trail_eq:
-  "do_skip_step S = S \<longleftrightarrow> trail (do_skip_step S) = trail S"
+lemma do_skip_step_eq_iff_raw_trail_eq:
+  "do_skip_step S = S \<longleftrightarrow> raw_trail (do_skip_step S) = raw_trail S"
   by (cases S rule: do_skip_step.cases) auto
 
-lemma do_decide_step_eq_iff_trail_eq:
-  "do_decide_step S = S \<longleftrightarrow> trail (do_decide_step S) = trail S"
+lemma do_decide_step_eq_iff_raw_trail_eq:
+  "do_decide_step S = S \<longleftrightarrow> raw_trail (do_decide_step S) = raw_trail S"
   by (cases S rule: do_decide_step.cases) (auto split: option.split)
 
-lemma do_backtrack_step_eq_iff_trail_eq:
-  assumes "no_dup (trail S)"
-  shows "do_backtrack_step S = S \<longleftrightarrow> raw_trail (do_backtrack_step S) = raw_trail S"
-  using assms apply (cases S rule: do_backtrack_step.cases)
-  by (auto split: option.split list.splits ann_lit.splits
-     simp: comp_def
-     dest!: bt_cut_in_get_all_ann_decomposition)
+lemma do_backtrack_step_eq_iff_raw_trail_eq:
+  "do_backtrack_step S = S \<longleftrightarrow> raw_trail (do_backtrack_step S) = raw_trail S"
+  by (cases S rule: do_backtrack_step.cases)
+     (auto split: option.split list.splits ann_lit.splits
+       dest!: bt_cut_in_get_all_decided_decomposition)
 
-lemma do_resolve_step_eq_iff_trail_eq:
-  "do_resolve_step S = S \<longleftrightarrow> trail (do_resolve_step S) = trail S"
+lemma do_resolve_step_eq_iff_raw_trail_eq:
+  "do_resolve_step S = S \<longleftrightarrow> raw_trail (do_resolve_step S) = raw_trail S"
   by (cases S rule: do_resolve_step.cases) auto
 
-lemma do_other_step_eq_iff_trail_eq:
-  assumes "no_dup (trail S)"
-  shows "do_other_step S = S \<longleftrightarrow> raw_trail (do_other_step S) = raw_trail S"
-  (* TODO proof *)
-  using assms
-  apply
-  (auto simp add: Let_def do_skip_step_eq_iff_trail_eq
-    do_decide_step_eq_iff_trail_eq do_backtrack_step_eq_iff_trail_eq
-    do_resolve_step_eq_iff_trail_eq
-    )
-  apply (simp add: do_resolve_step_eq_iff_trail_eq[symmetric]
-     do_skip_step_eq_iff_trail_eq[symmetric])
-  apply (simp add: do_skip_step_eq_iff_trail_eq[symmetric]
-    do_decide_step_eq_iff_trail_eq  do_backtrack_step_eq_iff_trail_eq[symmetric]
-    do_resolve_step_eq_iff_trail_eq[symmetric]
-    )
-  done
+lemma do_other_step_eq_iff_raw_trail_eq:
+  "raw_trail (do_other_step S) = raw_trail S \<longleftrightarrow> do_other_step S = S"
+  by (auto simp add: Let_def do_skip_step_eq_iff_raw_trail_eq[symmetric]
+    do_decide_step_eq_iff_raw_trail_eq[symmetric] do_backtrack_step_eq_iff_raw_trail_eq[symmetric]
+    do_resolve_step_eq_iff_raw_trail_eq[symmetric])
+
 
 lemma do_full1_cp_step_do_other_step'_normal_form[dest!]:
   assumes H: "do_full1_cp_step (do_other_step' S) = S"
   shows "do_other_step' S = S \<and> do_full1_cp_step S = S"
 proof -
   let ?T = "do_other_step' S"
-  { assume confl: "conc_conflicting (rough_state_of ?T) \<noteq> None"
-    then have tr: "trail (rough_state_of (do_full1_cp_step ?T)) = trail (rough_state_of ?T)"
-      using do_full1_cp_step_conflicting by fastforce
-    have "raw_trail (rough_state_of (do_full1_cp_step (do_other_step' S))) =
-      raw_trail (rough_state_of S)"
+  { assume confl: "raw_conflicting (rough_state_of ?T) \<noteq> None"
+    then have tr: "raw_trail (rough_state_of (do_full1_cp_step ?T)) = raw_trail (rough_state_of ?T)"
+      using do_full1_cp_step_raw_conflicting[of ?T] by auto
+    have "raw_trail (rough_state_of (do_full1_cp_step (do_other_step' S))) = raw_trail (rough_state_of S)"
       using arg_cong[OF H, of "\<lambda>S. raw_trail (rough_state_of S)"] .
     then have "raw_trail (rough_state_of (do_other_step' S)) = raw_trail (rough_state_of S)"
-       using confl by (auto simp add: do_full1_cp_step_conflicting)
-    moreover have "no_dup (trail (rough_state_of S))"
-      using rough_state_of[of S] unfolding cdcl\<^sub>W_all_struct_inv_def cdcl\<^sub>W_M_level_inv_def
-      by (cases S) (auto simp: comp_def)
-    ultimately have "do_other_step' S = S"
-      by (simp add: do_other_step_eq_iff_trail_eq[symmetric] do_other_step'_def
+       by (auto simp add: do_full1_cp_step_raw_conflicting confl)
+    then have "do_other_step' S = S"
+      by (simp add: do_other_step_eq_iff_raw_trail_eq do_other_step'_def
         del: do_other_step.simps)
   }
   moreover {
     assume eq[simp]: "do_other_step' S = S"
-    obtain c where c: "raw_trail (rough_state_of (do_full1_cp_step S)) =
-      c @ raw_trail (rough_state_of S)"
-      using do_full1_cp_step_neq_trail_increase by auto
+    obtain c where c: "raw_trail (rough_state_of (do_full1_cp_step S)) = c @ raw_trail (rough_state_of S)"
+      using do_full1_cp_step_neq_raw_trail_increase by auto
 
     moreover have "raw_trail (rough_state_of (do_full1_cp_step S)) = raw_trail (rough_state_of S)"
       using arg_cong[OF H, of "\<lambda>S. raw_trail (rough_state_of S)"] by simp
@@ -1306,18 +1286,17 @@ proof -
     then have "do_full1_cp_step S = S" using assms by auto
     }
   moreover {
-    assume confl: "conc_conflicting (rough_state_of ?T) = None" and neq: "do_other_step' S \<noteq> S"
+    assume confl: "raw_conflicting (rough_state_of ?T) = None" and neq: "do_other_step' S \<noteq> S"
     obtain c where
       c: "raw_trail (rough_state_of (do_full1_cp_step ?T)) = c @ raw_trail (rough_state_of ?T)" and
       nm: "\<forall>m\<in>set c. \<not> is_decided m"
-      using do_full1_cp_step_neq_trail_increase by auto
+      using do_full1_cp_step_neq_raw_trail_increase by auto
     have "length (filter is_decided (raw_trail (rough_state_of (do_full1_cp_step ?T))))
-       = length (filter is_decided (raw_trail (rough_state_of ?T)))"
-      using nm unfolding c by force
+       = length (filter is_decided (raw_trail (rough_state_of ?T)))" using nm unfolding c by force
     moreover have "length (filter is_decided (raw_trail (rough_state_of S)))
-       \<noteq> length (filter is_decided (raw_trail (rough_state_of ?T)))"
-      using do_other_step_not_conflicting_one_more_decide[OF _ neq]
-      do_other_step_not_conflicting_one_more_decide_bt[of S, OF _ confl neq]
+       \<noteq> length (filter is_decided  (raw_trail (rough_state_of ?T)))"
+      using do_other_step_not_raw_conflicting_one_more_decide[OF _ neq]
+      do_other_step_not_raw_conflicting_one_more_decide_bt[of S, OF _ confl neq]
       by linarith
     finally have False unfolding H by blast
   }
@@ -1326,20 +1305,20 @@ qed
 
 lemma do_cdcl\<^sub>W_stgy_step_no:
   assumes S: "do_cdcl\<^sub>W_stgy_step S = S"
-  shows "no_step cdcl\<^sub>W_stgy (rough_state_of S)"
+  shows "no_step cdcl\<^sub>W_stgy (toS (rough_state_of S))"
 proof -
   {
     fix S'
-    assume "full1 cdcl\<^sub>W_cp (rough_state_of S) S'"
+    assume "full1 cdcl\<^sub>W_cp (toS (rough_state_of S)) S'"
     then have False
       using do_full1_cp_step_full[of S] unfolding full_def S rtranclp_unfold full1_def
       by (smt assms do_cdcl\<^sub>W_stgy_step_def tranclpD)
   }
   moreover {
     fix S' S''
-    assume " cdcl\<^sub>W_o (rough_state_of S) S'" and
-     "no_step propagate (rough_state_of S)" and
-     "no_step conflict (rough_state_of S)" and
+    assume " cdcl\<^sub>W_o (toS (rough_state_of S)) S'" and
+     "no_step propagate (toS (rough_state_of S))" and
+     "no_step conflict (toS (rough_state_of S))" and
      "full cdcl\<^sub>W_cp S' S''"
     then have False
       using assms unfolding do_cdcl\<^sub>W_stgy_step_def
@@ -1350,8 +1329,8 @@ proof -
 qed
 
 lemma toS_rough_state_of_state_of_rough_state_from_init_state_of[simp]:
-  "rough_state_of (state_of (rough_state_from_init_state_of S))
-    = rough_state_from_init_state_of S"
+  "toS (rough_state_of (state_of (rough_state_from_init_state_of S)))
+    = toS (rough_state_from_init_state_of S)"
   using rough_state_from_init_state_of[of S] by (auto simp add: state_of_inverse)
 
 lemma cdcl\<^sub>W_cp_is_rtranclp_cdcl\<^sub>W: "cdcl\<^sub>W_cp S T \<Longrightarrow> cdcl\<^sub>W\<^sup>*\<^sup>* S T"
@@ -1370,92 +1349,34 @@ lemma cdcl\<^sub>W_stgy_is_rtranclp_cdcl\<^sub>W:
    using cdcl\<^sub>W_stgy.conflict' rtranclp_cdcl\<^sub>W_stgy_rtranclp_cdcl\<^sub>W apply blast
   unfolding full_def by (fastforce dest!:other rtranclp_cdcl\<^sub>W_cp_is_rtranclp_cdcl\<^sub>W)
 
-lemma cdcl\<^sub>W_stgy_init_clss: "cdcl\<^sub>W_stgy S T \<Longrightarrow> cdcl\<^sub>W_M_level_inv S \<Longrightarrow> init_clss S = init_clss T"
-  using rtranclp_cdcl\<^sub>W_init_clss cdcl\<^sub>W_stgy_is_rtranclp_cdcl\<^sub>W by fast
+lemma cdcl\<^sub>W_stgy_init_raw_init_clss: "cdcl\<^sub>W_stgy S T \<Longrightarrow> cdcl\<^sub>W_M_level_inv S \<Longrightarrow> raw_init_clss S = raw_init_clss T"
+  using rtranclp_cdcl\<^sub>W_init_raw_init_clss cdcl\<^sub>W_stgy_is_rtranclp_cdcl\<^sub>W by fast
 
 lemma clauses_toS_rough_state_of_do_cdcl\<^sub>W_stgy_step[simp]:
-  "init_clss (rough_state_of (do_cdcl\<^sub>W_stgy_step (state_of (rough_state_from_init_state_of S))))
-    = init_clss (rough_state_from_init_state_of S)" (is "_ = init_clss ?S")
-proof (cases "do_cdcl\<^sub>W_stgy_step (state_of ?S) = state_of ?S")
-  case True
-  then show ?thesis by simp
-next
-  case False
-  have "\<And>c. cdcl\<^sub>W_M_level_inv (rough_state_of c)"
-    using cdcl\<^sub>W_all_struct_inv_def cdcl\<^sub>W_all_struct_inv_rough_state by blast
-  then have "\<And>c. init_clss (rough_state_of c) = init_clss (rough_state_of (do_cdcl\<^sub>W_stgy_step c))
-    \<or> do_cdcl\<^sub>W_stgy_step c = c"
-    using cdcl\<^sub>W_stgy_no_more_init_clss do_cdcl\<^sub>W_stgy_step by blast
-  then show ?thesis
-    using False by force
-qed
-
-lemma raw_init_clss_do_cp_step[simp]:
-  "raw_init_clss (do_cp_step S) = raw_init_clss S"
- by (cases S) (auto simp: do_cp_step_def do_propagate_step_def do_conflict_step_def
-  split: option.splits)
-lemma raw_init_clss_do_cp_step'[simp]:
-  "raw_init_clss (rough_state_of (do_cp_step' S)) = raw_init_clss (rough_state_of S)"
-  by (simp add: do_cp_step'_def)
-
-lemma raw_init_clss_rough_state_of_do_full1_cp_step[simp]:
-  "raw_init_clss (rough_state_of (do_full1_cp_step S))
- = raw_init_clss (rough_state_of S)"
-  apply (rule do_full1_cp_step.induct[of "\<lambda>S.
-    raw_init_clss (rough_state_of (do_full1_cp_step S))
- = raw_init_clss (rough_state_of S)"])
-  by (metis (mono_tags, lifting) do_full1_cp_step.simps raw_init_clss_do_cp_step')
-
-lemma raw_init_clss_do_skip_def[simp]:
-  "raw_init_clss (do_skip_step S) = raw_init_clss S"
-  by (cases S rule: do_skip_step.cases) (auto simp: do_other_step'_def Let_def
-  split: option.splits)
-
-lemma raw_init_clss_do_resolve_def[simp]:
-  "raw_init_clss (do_resolve_step S) = raw_init_clss S"
-  by (cases S rule: do_resolve_step.cases) (auto simp: do_other_step'_def Let_def
-  split: option.splits)
-
-lemma raw_init_clss_do_backtrack_def[simp]:
-  "raw_init_clss (do_backtrack_step S) = raw_init_clss S"
-  by (cases S rule: do_backtrack_step.cases) (auto simp: do_other_step'_def Let_def
-  split: option.splits list.splits ann_lit.splits)
-
-
-lemma raw_init_clss_do_decide_def[simp]:
-  "raw_init_clss (do_decide_step S) = raw_init_clss S"
-  by (cases S rule: do_decide_step.cases) (auto simp: do_other_step'_def Let_def
-   split: option.splits)
-
-lemma raw_init_clss_rough_state_of_do_other_step'[simp]:
-  "raw_init_clss (rough_state_of (do_other_step' S))
-  = raw_init_clss (rough_state_of S)"
-  by (cases S) (auto simp: do_other_step'_def Let_def do_skip_step.cases
-  split: option.splits)
-
-lemma [simp]:
-  "raw_init_clss (rough_state_of (do_cdcl\<^sub>W_stgy_step (state_of (rough_state_from_init_state_of S))))
-  =
-  raw_init_clss (rough_state_from_init_state_of S)"
-  unfolding do_cdcl\<^sub>W_stgy_step_def by (auto simp: Let_def)
+  "raw_init_clss (toS (rough_state_of (do_cdcl\<^sub>W_stgy_step (state_of (rough_state_from_init_state_of S)))))
+    = raw_init_clss (toS (rough_state_from_init_state_of S))" (is "_ = raw_init_clss (toS ?S)")
+  apply (cases "do_cdcl\<^sub>W_stgy_step (state_of ?S) = state_of ?S")
+    apply simp
+  by (smt cdcl\<^sub>W_all_struct_inv_def cdcl\<^sub>W_all_struct_inv_rough_state cdcl\<^sub>W_stgy_no_more_init_raw_init_clss
+    do_cdcl\<^sub>W_stgy_step toS_rough_state_of_state_of_rough_state_from_init_state_of)
 
 lemma rough_state_from_init_state_of_do_cdcl\<^sub>W_stgy_step'[code abstract]:
  "rough_state_from_init_state_of (do_cdcl\<^sub>W_stgy_step' S) =
    rough_state_of (do_cdcl\<^sub>W_stgy_step (id_of_I_to S))"
 proof -
-  let ?S = "rough_state_from_init_state_of S"
-  have "cdcl\<^sub>W_stgy\<^sup>*\<^sup>* (raw_S0_cdcl\<^sub>W (raw_init_clss (rough_state_from_init_state_of S)))
-    (rough_state_from_init_state_of S)"
+  let ?S = "(rough_state_from_init_state_of S)"
+  have "cdcl\<^sub>W_stgy\<^sup>*\<^sup>* (S0_cdcl\<^sub>W (raw_init_clss (toS (rough_state_from_init_state_of S))))
+    (toS (rough_state_from_init_state_of S))"
     using rough_state_from_init_state_of[of S] by auto
   moreover have "cdcl\<^sub>W_stgy\<^sup>*\<^sup>*
-                  (rough_state_from_init_state_of S)
-                  (rough_state_of (do_cdcl\<^sub>W_stgy_step
-                    (state_of (rough_state_from_init_state_of S))))"
+                  (toS (rough_state_from_init_state_of S))
+                  (toS (rough_state_of (do_cdcl\<^sub>W_stgy_step
+                    (state_of (rough_state_from_init_state_of S)))))"
      using do_cdcl\<^sub>W_stgy_step[of "state_of ?S"]
      by (cases "do_cdcl\<^sub>W_stgy_step (state_of ?S) = state_of ?S") auto
   ultimately show ?thesis
     unfolding do_cdcl\<^sub>W_stgy_step'_def id_of_I_to_def
-    by (auto intro: state_from_init_state_of_inverse)
+    by (auto intro!: state_from_init_state_of_inverse)
 qed
 
 paragraph \<open>All rules together\<close>
@@ -1466,39 +1387,38 @@ function do_all_cdcl\<^sub>W_stgy where
 by fast+
 termination
 proof (relation "{(T, S).
-    (cdcl\<^sub>W_measure (rough_state_from_init_state_of T),
-    cdcl\<^sub>W_measure (rough_state_from_init_state_of S))
-      \<in> lexn less_than 3}", goal_cases)
+    (cdcl\<^sub>W_measure (toS (rough_state_from_init_state_of T)),
+    cdcl\<^sub>W_measure (toS (rough_state_from_init_state_of S)))
+      \<in> lexn {(a, b). a < b} 3}", goal_cases)
   case 1
   show ?case by (rule wf_if_measure_f) (auto intro!: wf_lexn wf_less)
 next
   case (2 S T) note T = this(1) and ST = this(2)
   let ?S = "rough_state_from_init_state_of S"
-  have S: "cdcl\<^sub>W_stgy\<^sup>*\<^sup>* (raw_S0_cdcl\<^sub>W (raw_init_clss ?S)) ?S"
+  have S: "cdcl\<^sub>W_stgy\<^sup>*\<^sup>* (S0_cdcl\<^sub>W (raw_init_clss (toS ?S))) (toS ?S)"
     using rough_state_from_init_state_of[of S] by auto
-  moreover have "cdcl\<^sub>W_stgy (rough_state_from_init_state_of S)
-    (rough_state_from_init_state_of T)"
-
+  moreover have "cdcl\<^sub>W_stgy (toS (rough_state_from_init_state_of S))
+    (toS (rough_state_from_init_state_of T))"
     proof -
       have "\<And>c. rough_state_of (state_of (rough_state_from_init_state_of c)) =
         rough_state_from_init_state_of c"
         using rough_state_from_init_state_of by force
       then have "do_cdcl\<^sub>W_stgy_step (state_of (rough_state_from_init_state_of S))
         \<noteq> state_of (rough_state_from_init_state_of S)"
-        using ST T  rough_state_from_init_state_of_inverse
-        unfolding id_of_I_to_def do_cdcl\<^sub>W_stgy_step'_def
+        using ST T by (metis (no_types) id_of_I_to_def rough_state_from_init_state_of_inject
+          rough_state_from_init_state_of_do_cdcl\<^sub>W_stgy_step')
+      then show ?thesis
+        using do_cdcl\<^sub>W_stgy_step id_of_I_to_def rough_state_from_init_state_of_do_cdcl\<^sub>W_stgy_step' T
         by fastforce
-      from do_cdcl\<^sub>W_stgy_step[OF this] show ?thesis
-        by (simp add: T id_of_I_to_def rough_state_from_init_state_of_do_cdcl\<^sub>W_stgy_step')
     qed
   moreover
-    have "cdcl\<^sub>W_all_struct_inv (rough_state_from_init_state_of S)"
+    have "cdcl\<^sub>W_all_struct_inv (toS (rough_state_from_init_state_of S))"
       using rough_state_from_init_state_of[of S] by auto
-    then have "cdcl\<^sub>W_all_struct_inv (raw_S0_cdcl\<^sub>W (raw_init_clss (rough_state_from_init_state_of S)))"
+    then have "cdcl\<^sub>W_all_struct_inv (S0_cdcl\<^sub>W (raw_init_clss (toS (rough_state_from_init_state_of S))))"
       by (cases "rough_state_from_init_state_of S")
          (auto simp add: cdcl\<^sub>W_all_struct_inv_def distinct_cdcl\<^sub>W_state_def)
   ultimately show ?case
-    by (auto intro!: cdcl\<^sub>W_stgy_step_decreasing[of _ _ "raw_S0_cdcl\<^sub>W (raw_init_clss ?S)"]
+    by (auto intro!: cdcl\<^sub>W_stgy_step_decreasing[of _ _ "S0_cdcl\<^sub>W (raw_init_clss (toS ?S))"]
       simp del: cdcl\<^sub>W_measure.simps)
 qed
 
@@ -1507,45 +1427,36 @@ lemma do_all_cdcl\<^sub>W_stgy_induct:
   "(\<And>S. (do_cdcl\<^sub>W_stgy_step' S \<noteq> S \<Longrightarrow> P (do_cdcl\<^sub>W_stgy_step' S)) \<Longrightarrow> P S) \<Longrightarrow> P a0"
  using do_all_cdcl\<^sub>W_stgy.induct by metis
 
-lemma [simp]: "raw_init_clss (rough_state_from_init_state_of (do_all_cdcl\<^sub>W_stgy S)) =
-  raw_init_clss (rough_state_from_init_state_of S)"
-  apply (induction rule: do_all_cdcl\<^sub>W_stgy_induct)
-  by (smt do_all_cdcl\<^sub>W_stgy.simps do_cdcl\<^sub>W_stgy_step_def id_of_I_to_def
-    raw_init_clss_rough_state_of_do_full1_cp_step raw_init_clss_rough_state_of_do_other_step'
-    rough_state_from_init_state_of_do_cdcl\<^sub>W_stgy_step'
-    toS_rough_state_of_state_of_rough_state_from_init_state_of)
-
 lemma no_step_cdcl\<^sub>W_stgy_cdcl\<^sub>W_all:
-  fixes S :: "'a cdcl\<^sub>W_state_inv_from_init_state"
-  shows "no_step cdcl\<^sub>W_stgy (rough_state_from_init_state_of (do_all_cdcl\<^sub>W_stgy S))"
+  "no_step cdcl\<^sub>W_stgy (toS (rough_state_from_init_state_of (do_all_cdcl\<^sub>W_stgy S)))"
   apply (induction S rule:do_all_cdcl\<^sub>W_stgy_induct)
   apply (rename_tac S, case_tac "do_cdcl\<^sub>W_stgy_step' S \<noteq> S")
 proof -
-  fix Sa :: "'a cdcl\<^sub>W_state_inv_from_init_state"
+  fix Sa :: cdcl\<^sub>W_state_inv_from_init_state
   assume a1: "\<not> do_cdcl\<^sub>W_stgy_step' Sa \<noteq> Sa"
   { fix pp
     have "(if True then Sa else do_all_cdcl\<^sub>W_stgy Sa) = do_all_cdcl\<^sub>W_stgy Sa"
       using a1 by auto
-    then have "\<not> cdcl\<^sub>W_stgy (rough_state_from_init_state_of (do_all_cdcl\<^sub>W_stgy Sa)) pp"
-      using a1 by (smt do_cdcl\<^sub>W_stgy_step_no id_of_I_to_def
+    then have "\<not> cdcl\<^sub>W_stgy (toS (rough_state_from_init_state_of (do_all_cdcl\<^sub>W_stgy Sa))) pp"
+      using a1 by (metis (no_types) do_cdcl\<^sub>W_stgy_step_no id_of_I_to_def
         rough_state_from_init_state_of_do_cdcl\<^sub>W_stgy_step' rough_state_of_inverse) }
-  then show "no_step cdcl\<^sub>W_stgy (rough_state_from_init_state_of (do_all_cdcl\<^sub>W_stgy Sa))"
+  then show "no_step cdcl\<^sub>W_stgy (toS (rough_state_from_init_state_of (do_all_cdcl\<^sub>W_stgy Sa)))"
     by fastforce
 next
-  fix Sa :: "'a cdcl\<^sub>W_state_inv_from_init_state"
+  fix Sa :: cdcl\<^sub>W_state_inv_from_init_state
   assume a1: "do_cdcl\<^sub>W_stgy_step' Sa \<noteq> Sa
-    \<Longrightarrow> no_step cdcl\<^sub>W_stgy (rough_state_from_init_state_of
-      (do_all_cdcl\<^sub>W_stgy (do_cdcl\<^sub>W_stgy_step' Sa)))"
+    \<Longrightarrow> no_step cdcl\<^sub>W_stgy (toS (rough_state_from_init_state_of
+      (do_all_cdcl\<^sub>W_stgy (do_cdcl\<^sub>W_stgy_step' Sa))))"
   assume a2: "do_cdcl\<^sub>W_stgy_step' Sa \<noteq> Sa"
   have "do_all_cdcl\<^sub>W_stgy Sa = do_all_cdcl\<^sub>W_stgy (do_cdcl\<^sub>W_stgy_step' Sa)"
     by (metis (full_types) do_all_cdcl\<^sub>W_stgy.simps)
-  then show "no_step cdcl\<^sub>W_stgy (rough_state_from_init_state_of (do_all_cdcl\<^sub>W_stgy Sa))"
+  then show "no_step cdcl\<^sub>W_stgy (toS (rough_state_from_init_state_of (do_all_cdcl\<^sub>W_stgy Sa)))"
     using a2 a1 by presburger
 qed
 
 lemma do_all_cdcl\<^sub>W_stgy_is_rtranclp_cdcl\<^sub>W_stgy:
-  "cdcl\<^sub>W_stgy\<^sup>*\<^sup>* (rough_state_from_init_state_of S)
-    (rough_state_from_init_state_of (do_all_cdcl\<^sub>W_stgy S))"
+  "cdcl\<^sub>W_stgy\<^sup>*\<^sup>* (toS (rough_state_from_init_state_of S))
+    (toS (rough_state_from_init_state_of (do_all_cdcl\<^sub>W_stgy S)))"
 proof (induction S rule: do_all_cdcl\<^sub>W_stgy_induct)
   case (1 S) note IH = this(1)
   show ?case
@@ -1557,101 +1468,77 @@ proof (induction S rule: do_all_cdcl\<^sub>W_stgy_induct)
       have f2: "do_cdcl\<^sub>W_stgy_step (id_of_I_to S) = id_of_I_to S \<longrightarrow>
         rough_state_from_init_state_of (do_cdcl\<^sub>W_stgy_step' S)
         = rough_state_of (state_of (rough_state_from_init_state_of S))"
-        unfolding  rough_state_from_init_state_of_do_cdcl\<^sub>W_stgy_step'
-        id_of_I_to_def by presburger
+        using id_of_I_to_def rough_state_from_init_state_of_do_cdcl\<^sub>W_stgy_step' by presburger
       have f3: "do_all_cdcl\<^sub>W_stgy S = do_all_cdcl\<^sub>W_stgy (do_cdcl\<^sub>W_stgy_step' S)"
         by (metis (full_types) do_all_cdcl\<^sub>W_stgy.simps)
-      have "cdcl\<^sub>W_stgy (rough_state_from_init_state_of S)
-          (rough_state_from_init_state_of (do_cdcl\<^sub>W_stgy_step' S))
-        = cdcl\<^sub>W_stgy (rough_state_of (id_of_I_to S))
-          (rough_state_of (do_cdcl\<^sub>W_stgy_step (id_of_I_to S)))"
-        unfolding id_of_I_to_def rough_state_from_init_state_of_do_cdcl\<^sub>W_stgy_step'
+      have "cdcl\<^sub>W_stgy (toS (rough_state_from_init_state_of S))
+          (toS (rough_state_from_init_state_of (do_cdcl\<^sub>W_stgy_step' S)))
+        = cdcl\<^sub>W_stgy (toS (rough_state_of (id_of_I_to S)))
+          (toS (rough_state_of (do_cdcl\<^sub>W_stgy_step (id_of_I_to S))))"
+        using id_of_I_to_def rough_state_from_init_state_of_do_cdcl\<^sub>W_stgy_step'
         toS_rough_state_of_state_of_rough_state_from_init_state_of by presburger
       then show ?thesis
-        using f3 f2 IH do_cdcl\<^sub>W_stgy_step
-        by (smt False toS_rough_state_of_state_of_rough_state_from_init_state_of tranclp.intros(1)
-          tranclp_into_rtranclp transitive_closurep_trans'(2))
+        using f3 f2 IH do_cdcl\<^sub>W_stgy_step by fastforce
     qed
 qed
 
 text \<open>Final theorem:\<close>
-lemma consistent_interp_mmset_of_mlit[simp]:
-  "consistent_interp (lit_of ` mmset_of_mlit' ` set M') \<longleftrightarrow>
-   consistent_interp (lit_of ` set M')"
-  by (auto simp: image_image)
-
 lemma DPLL_tot_correct:
   assumes
     r: "rough_state_from_init_state_of (do_all_cdcl\<^sub>W_stgy (state_from_init_state_of
       (([], map remdups N, [], 0, None)))) = S" and
-    S: "(M', N', U', k, E) = S"
-  shows "(E \<noteq> Some [] \<and> satisfiable (set (map mset N)))
-    \<or> (E = Some [] \<and> unsatisfiable (set (map mset N)))"
+    S: "(M', N', U', k, E) = toS S"
+  shows "(E \<noteq> Some {#} \<and> satisfiable (set (map mset N)))
+    \<or> (E = Some {#} \<and> unsatisfiable (set (map mset N)))"
 proof -
   let ?N = "map remdups N"
-  have inv: "cdcl\<^sub>W_all_struct_inv ([], map remdups N, [], 0, None)"
+  have inv: "cdcl\<^sub>W_all_struct_inv (toS ([], map remdups N, [], 0, None))"
     unfolding cdcl\<^sub>W_all_struct_inv_def distinct_cdcl\<^sub>W_state_def distinct_mset_set_def by auto
   then have S0: "rough_state_of (state_of ([], map remdups N, [], 0, None))
     = ([], map remdups N, [], 0, None)" by simp
-  have 1: "full cdcl\<^sub>W_stgy ([], ?N, [], 0, None) S"
+  have 1: "full cdcl\<^sub>W_stgy (toS ([], ?N, [], 0, None)) (toS S)"
     unfolding full_def apply rule
       using do_all_cdcl\<^sub>W_stgy_is_rtranclp_cdcl\<^sub>W_stgy[of
         "state_from_init_state_of ([], map remdups N, [], 0, None)"] inv
+        no_step_cdcl\<^sub>W_stgy_cdcl\<^sub>W_all
         by (auto simp del: do_all_cdcl\<^sub>W_stgy.simps simp: state_from_init_state_of_inverse
-          r[symmetric] no_step_cdcl\<^sub>W_stgy_cdcl\<^sub>W_all)+
+          r[symmetric])+
   moreover have 2: "finite (set (map mset ?N))" by auto
   moreover have 3: "distinct_mset_set (set (map mset ?N))"
      unfolding distinct_mset_set_def by auto
   moreover
-    have "cdcl\<^sub>W_all_struct_inv S"
+    have "cdcl\<^sub>W_all_struct_inv (toS S)"
       by (metis (no_types) cdcl\<^sub>W_all_struct_inv_rough_state r
         toS_rough_state_of_state_of_rough_state_from_init_state_of)
-    then have cons: "consistent_interp (lits_of_l M')"
-      unfolding cdcl\<^sub>W_all_struct_inv_def cdcl\<^sub>W_M_level_inv_def S[symmetric]
-      by (auto simp: lits_of_def)
+    then have cons: "consistent_interp (lits_of M')"
+      unfolding cdcl\<^sub>W_all_struct_inv_def cdcl\<^sub>W_M_level_inv_def S[symmetric] by auto
   moreover
-    have [simp]:
-      "rough_state_from_init_state_of (state_from_init_state_of (raw_S0_cdcl\<^sub>W (map remdups N)))
-      = raw_S0_cdcl\<^sub>W (map remdups N)"
-      apply (rule cdcl\<^sub>W_state_inv_from_init_state.state_from_init_state_of_inverse)
-      using 3 by (auto simp: cdcl\<^sub>W_all_struct_inv_def distinct_cdcl\<^sub>W_state_def
-        image_image comp_def)
-    have "raw_init_clss ([], ?N, [], 0, None) = raw_init_clss S"
-      using arg_cong[OF r, of raw_init_clss] unfolding S[symmetric]
-      by (simp del: do_all_cdcl\<^sub>W_stgy.simps)
-    then have N': "N' =map remdups N"
+    have "raw_init_clss (toS ([], ?N, [], 0, None)) = raw_init_clss (toS S)"
+      apply (rule rtranclp_cdcl\<^sub>W_init_raw_init_clss)
+      using 1 unfolding full_def by (auto simp add: rtranclp_cdcl\<^sub>W_stgy_rtranclp_cdcl\<^sub>W)
+    then have N': "mset (map mset ?N) = N'"
       using S[symmetric] by auto
-
-  have "conc_conflicting S = Some {#} \<and> unsatisfiable (set_mset (init_clss S)) \<or>
-    conflicting S = None \<and> (case S of (M, uu_) \<Rightarrow> map mmset_of_mlit' M) \<Turnstile>asm init_clss S"
-    apply (rule full_cdcl\<^sub>W_stgy_final_state_conclusive)
+  have "(E \<noteq> Some {#} \<and> satisfiable (set (map mset ?N)))
+    \<or> (E = Some {#} \<and> unsatisfiable (set (map mset ?N)))"
+    using full_cdcl\<^sub>W_stgy_final_state_conclusive unfolding N' apply rule
         using 1 apply simp
        using 2 apply simp
-      using 3 by simp
-  then have "(E \<noteq> Some [] \<and> satisfiable (set (map mset ?N)))
-    \<or> (E = Some [] \<and> unsatisfiable (set (map mset ?N)))"
-    using cons unfolding S[symmetric] N' apply (auto simp: comp_def)
-    by (simp add: true_annots_true_cls)
+      using 3 apply simp
+     using S[symmetric] N' apply auto[1]
+   using S[symmetric] N' cons by (fastforce simp: true_annots_true_cls)
   then show ?thesis by auto
 qed
 
 paragraph \<open>The Code\<close>
 text \<open>The SML code is skipped in the documentation, but stays to ensure that some version of the
  exported code is working. The only difference between the generated code and the one used here is
- the export of the constructor ConI (such that we can use it).\<close>
-
+ the export of the constructor ConI.\<close>
 (*<*)
 fun gene where
 "gene 0 = [[Pos 0], [Neg 0]]" |
 "gene (Suc n) = map (op # (Pos (Suc n))) (gene n) @ map (op # (Neg (Suc n))) (gene n)"
 
 value "gene 1"
-
-text \<open>@{term maximum_level_code} and @{term get_level} have to be declared in the same module.
-  Otherwise, the code-generator complains about cyclic dependency.\<close>
-code_identifier
- code_module CDCL_W_Level \<rightharpoonup> (SML) CDCL_W_Level |
- code_module DPLL_CDCL_W_Implementation \<rightharpoonup> (SML) CDCL_W_Level
 
 export_code do_all_cdcl\<^sub>W_stgy gene in SML
 ML \<open>
@@ -1668,70 +1555,10 @@ fun eq A_ a b = equal A_ a b;
 
 end; (*struct HOL*)
 
-structure Orderings : sig
-  type 'a ord
-  val less_eq : 'a ord -> 'a -> 'a -> bool
-  val less : 'a ord -> 'a -> 'a -> bool
-  val max : 'a ord -> 'a -> 'a -> 'a
-end = struct
-
-type 'a ord = {less_eq : 'a -> 'a -> bool, less : 'a -> 'a -> bool};
-val less_eq = #less_eq : 'a ord -> 'a -> 'a -> bool;
-val less = #less : 'a ord -> 'a -> 'a -> bool;
-
-fun max A_ a b = (if less_eq A_ a b then b else a);
-
-end; (*struct Orderings*)
-
-structure Arith : sig
-  datatype nat = Zero_nat | Suc of nat
-  val equal_nata : nat -> nat -> bool
-  val equal_nat : nat HOL.equal
-  type 'a one
-  val one : 'a one -> 'a
-  val one_nat : nat one
-  type 'a plus
-  val plus : 'a plus -> 'a -> 'a -> 'a
-  val plus_nat : nat plus
-  val less_nat : nat -> nat -> bool
-  val ord_nat : nat Orderings.ord
-end = struct
-
-datatype nat = Zero_nat | Suc of nat;
-
-fun equal_nata Zero_nat (Suc x2) = false
-  | equal_nata (Suc x2) Zero_nat = false
-  | equal_nata (Suc x2) (Suc y2) = equal_nata x2 y2
-  | equal_nata Zero_nat Zero_nat = true;
-
-val equal_nat = {equal = equal_nata} : nat HOL.equal;
-
-val one_nata : nat = Suc Zero_nat;
-
-type 'a one = {one : 'a};
-val one = #one : 'a one -> 'a;
-
-val one_nat = {one = one_nata} : nat one;
-
-fun plus_nata (Suc m) n = plus_nata m (Suc n)
-  | plus_nata Zero_nat n = n;
-
-type 'a plus = {plus : 'a -> 'a -> 'a};
-val plus = #plus : 'a plus -> 'a -> 'a -> 'a;
-
-val plus_nat = {plus = plus_nata} : nat plus;
-
-fun less_eq_nat (Suc m) n = less_nat m n
-  | less_eq_nat Zero_nat n = true
-and less_nat m (Suc n) = less_eq_nat m n
-  | less_nat n Zero_nat = false;
-
-val ord_nat = {less_eq = less_eq_nat, less = less_nat} : nat Orderings.ord;
-
-end; (*struct Arith*)
-
 structure List : sig
   val equal_list : 'a HOL.equal -> ('a list) HOL.equal
+  val fold : ('a -> 'b -> 'b) -> 'a list -> 'b -> 'b
+  val rev : 'a list -> 'a list
   val find : ('a -> bool) -> 'a list -> 'a option
   val null : 'a list -> bool
   val filter : ('a -> bool) -> 'a list -> 'a list
@@ -1739,9 +1566,7 @@ structure List : sig
   val remdups : 'a HOL.equal -> 'a list -> 'a list
   val remove1 : 'a HOL.equal -> 'a -> 'a list -> 'a list
   val map : ('a -> 'b) -> 'a list -> 'b list
-  val dropWhile : ('a -> bool) -> 'a list -> 'a list
   val list_all : ('a -> bool) -> 'a list -> bool
-  val size_list : 'a list -> Arith.nat
 end = struct
 
 fun equal_lista A_ [] (x21 :: x22) = false
@@ -1751,6 +1576,11 @@ fun equal_lista A_ [] (x21 :: x22) = false
   | equal_lista A_ [] [] = true;
 
 fun equal_list A_ = {equal = equal_lista A_} : ('a list) HOL.equal;
+
+fun fold f (x :: xs) s = fold f xs (f x s)
+  | fold f [] s = s;
+
+fun rev xs = fold (fn a => fn b => a :: b) xs [];
 
 fun find uu [] = NONE
   | find p (x :: xs) = (if p x then SOME x else find p xs);
@@ -1775,16 +1605,8 @@ fun remove1 A_ x [] = []
 fun map f [] = []
   | map f (x21 :: x22) = f x21 :: map f x22;
 
-fun dropWhile p [] = []
-  | dropWhile p (x :: xs) = (if p x then dropWhile p xs else x :: xs);
-
-fun gen_length n (x :: xs) = gen_length (Arith.Suc n) xs
-  | gen_length n [] = n;
-
 fun list_all p [] = true
   | list_all p (x :: xs) = p x andalso list_all p xs;
-
-fun size_list x = gen_length Arith.Zero_nat x;
 
 end; (*struct List*)
 
@@ -1803,6 +1625,75 @@ fun member A_ x (Coset xs) = not (List.member A_ xs x)
 
 end; (*struct Set*)
 
+structure Orderings : sig
+  type 'a ord
+  val less_eq : 'a ord -> 'a -> 'a -> bool
+  val less : 'a ord -> 'a -> 'a -> bool
+  type 'a preorder
+  val ord_preorder : 'a preorder -> 'a ord
+  type 'a order
+  val preorder_order : 'a order -> 'a preorder
+  type 'a linorder
+  val order_linorder : 'a linorder -> 'a order
+  val max : 'a ord -> 'a -> 'a -> 'a
+end = struct
+
+type 'a ord = {less_eq : 'a -> 'a -> bool, less : 'a -> 'a -> bool};
+val less_eq = #less_eq : 'a ord -> 'a -> 'a -> bool;
+val less = #less : 'a ord -> 'a -> 'a -> bool;
+
+type 'a preorder = {ord_preorder : 'a ord};
+val ord_preorder = #ord_preorder : 'a preorder -> 'a ord;
+
+type 'a order = {preorder_order : 'a preorder};
+val preorder_order = #preorder_order : 'a order -> 'a preorder;
+
+type 'a linorder = {order_linorder : 'a order};
+val order_linorder = #order_linorder : 'a linorder -> 'a order;
+
+fun max A_ a b = (if less_eq A_ a b then b else a);
+
+end; (*struct Orderings*)
+
+structure Arith : sig
+  datatype nat = Zero_nat | Suc of nat
+  val equal_nata : nat -> nat -> bool
+  val equal_nat : nat HOL.equal
+  val less_nat : nat -> nat -> bool
+  val linorder_nat : nat Orderings.linorder
+  val one_nat : nat
+  val plus_nat : nat -> nat -> nat
+end = struct
+
+datatype nat = Zero_nat | Suc of nat;
+
+fun equal_nata Zero_nat (Suc x2) = false
+  | equal_nata (Suc x2) Zero_nat = false
+  | equal_nata (Suc x2) (Suc y2) = equal_nata x2 y2
+  | equal_nata Zero_nat Zero_nat = true;
+
+val equal_nat = {equal = equal_nata} : nat HOL.equal;
+
+fun less_eq_nat (Suc m) n = less_nat m n
+  | less_eq_nat Zero_nat n = true
+and less_nat m (Suc n) = less_eq_nat m n
+  | less_nat n Zero_nat = false;
+
+val ord_nat = {less_eq = less_eq_nat, less = less_nat} : nat Orderings.ord;
+
+val preorder_nat = {ord_preorder = ord_nat} : nat Orderings.preorder;
+
+val order_nat = {preorder_order = preorder_nat} : nat Orderings.order;
+
+val linorder_nat = {order_linorder = order_nat} : nat Orderings.linorder;
+
+val one_nat : nat = Suc Zero_nat;
+
+fun plus_nat (Suc m) n = plus_nat m (Suc n)
+  | plus_nat Zero_nat n = n;
+
+end; (*struct Arith*)
+
 structure Option : sig
   val equal_option : 'a HOL.equal -> ('a option) HOL.equal
 end = struct
@@ -1818,9 +1709,21 @@ end; (*struct Option*)
 
 structure Multiset : sig
   datatype 'a multiset = Mset of 'a list
+  val single : 'a -> 'a multiset
+  val set_mset : 'a multiset -> 'a Set.set
+  val image_mset : ('a -> 'b) -> 'a multiset -> 'b multiset
+  val plus_multiset : 'a multiset -> 'a multiset -> 'a multiset
 end = struct
 
 datatype 'a multiset = Mset of 'a list;
+
+fun single x = Mset [x];
+
+fun set_mset (Mset x) = Set.Set x;
+
+fun image_mset f (Mset xs) = Mset (List.map f xs);
+
+fun plus_multiset (Mset xs) (Mset ys) = Mset (xs @ ys);
 
 end; (*struct Multiset*)
 
@@ -1852,36 +1755,79 @@ fun uminus_literal l = (if is_pos l then Neg else Pos) (atm_of l);
 end; (*struct Clausal_Logic*)
 
 structure Partial_Annotated_Clausal_Logic : sig
-  datatype ('a, 'b) ann_lit = Decided of 'a Clausal_Logic.literal |
-    Propagated of 'a Clausal_Logic.literal * 'b
-  val equal_ann_lit : 'a HOL.equal -> 'b HOL.equal -> ('a, 'b) ann_lit HOL.equal
-  val lit_of : ('a, 'b) ann_lit -> 'a Clausal_Logic.literal
-  val lits_of : ('a, 'b) ann_lit Set.set -> 'a Clausal_Logic.literal Set.set
-  val is_decided : ('a, 'b) ann_lit -> bool
+  datatype ('a, 'b, 'c) ann_lit = Decided of 'a Clausal_Logic.literal * 'b |
+    Propagated of 'a Clausal_Logic.literal * 'c
+  val equal_ann_lit :
+    'a HOL.equal -> 'b HOL.equal -> 'c HOL.equal ->
+      ('a, 'b, 'c) ann_lit HOL.equal
+  val lits_of : ('a, 'b, 'c) ann_lit list -> 'a Clausal_Logic.literal Set.set
 end = struct
 
-datatype ('a, 'b) ann_lit = Decided of 'a Clausal_Logic.literal |
-  Propagated of 'a Clausal_Logic.literal * 'b;
+datatype ('a, 'b, 'c) ann_lit = Decided of 'a Clausal_Logic.literal * 'b |
+  Propagated of 'a Clausal_Logic.literal * 'c;
 
-fun equal_ann_lita A_ B_ (Decided x1) (Propagated (x21, x22)) = false
-  | equal_ann_lita A_ B_ (Propagated (x21, x22)) (Decided x1) = false
-  | equal_ann_lita A_ B_ (Propagated (x21, x22)) (Propagated (y21, y22)) =
-    Clausal_Logic.equal_literala A_ x21 y21 andalso HOL.eq B_ x22 y22
-  | equal_ann_lita A_ B_ (Decided x1) (Decided y1) =
-    Clausal_Logic.equal_literala A_ x1 y1;
+fun equal_ann_lita A_ B_ C_ (Decided (x11, x12)) (Propagated (x21, x22)) =
+  false
+  | equal_ann_lita A_ B_ C_ (Propagated (x21, x22)) (Decided (x11, x12)) =
+    false
+  | equal_ann_lita A_ B_ C_ (Propagated (x21, x22)) (Propagated (y21, y22)) =
+    Clausal_Logic.equal_literala A_ x21 y21 andalso HOL.eq C_ x22 y22
+  | equal_ann_lita A_ B_ C_ (Decided (x11, x12)) (Decided (y11, y12)) =
+    Clausal_Logic.equal_literala A_ x11 y11 andalso HOL.eq B_ x12 y12;
 
-fun equal_ann_lit A_ B_ = {equal = equal_ann_lita A_ B_} :
-  ('a, 'b) ann_lit HOL.equal;
+fun equal_ann_lit A_ B_ C_ = {equal = equal_ann_lita A_ B_ C_} :
+  ('a, 'b, 'c) ann_lit HOL.equal;
 
-fun lit_of (Decided x1) = x1
+fun lit_of (Decided (x11, x12)) = x11
   | lit_of (Propagated (x21, x22)) = x21;
 
-fun lits_of ls = Set.image lit_of ls;
-
-fun is_decided (Decided x1) = true
-  | is_decided (Propagated (x21, x22)) = false;
+fun lits_of ls = Set.image lit_of (Set.Set ls);
 
 end; (*struct Partial_Annotated_Clausal_Logic*)
+
+structure Lattices_Big : sig
+  val max : 'a Orderings.linorder -> 'a Set.set -> 'a
+end = struct
+
+fun max A_ (Set.Set (x :: xs)) =
+  List.fold
+    (Orderings.max
+      ((Orderings.ord_preorder o Orderings.preorder_order o
+         Orderings.order_linorder)
+        A_))
+    xs x;
+
+end; (*struct Lattices_Big*)
+
+structure CDCL_W_Level : sig
+  val get_rev_level :
+    'a HOL.equal ->
+      ('a, Arith.nat, 'b) Partial_Annotated_Clausal_Logic.ann_lit list ->
+        Arith.nat -> 'a Clausal_Logic.literal -> Arith.nat
+  val get_maximum_level :
+    'a HOL.equal ->
+      ('a, Arith.nat, 'b) Partial_Annotated_Clausal_Logic.ann_lit list ->
+        'a Clausal_Logic.literal Multiset.multiset -> Arith.nat
+end = struct
+
+fun get_rev_level A_ [] uu uv = Arith.Zero_nat
+  | get_rev_level A_ (Partial_Annotated_Clausal_Logic.Decided (la, level) :: ls)
+    n l =
+    (if HOL.eq A_ (Clausal_Logic.atm_of la) (Clausal_Logic.atm_of l) then level
+      else get_rev_level A_ ls level l)
+  | get_rev_level A_ (Partial_Annotated_Clausal_Logic.Propagated (la, uw) :: ls)
+    n l =
+    (if HOL.eq A_ (Clausal_Logic.atm_of la) (Clausal_Logic.atm_of l) then n
+      else get_rev_level A_ ls n l);
+
+fun get_maximum_level A_ m d =
+  Lattices_Big.max Arith.linorder_nat
+    (Multiset.set_mset
+      (Multiset.plus_multiset (Multiset.single Arith.Zero_nat)
+        (Multiset.image_mset (get_rev_level A_ (List.rev m) Arith.Zero_nat)
+          d)));
+
+end; (*struct CDCL_W_Level*)
 
 structure Product_Type : sig
   val equal_proda : 'a HOL.equal -> 'b HOL.equal -> 'a * 'b -> 'a * 'b -> bool
@@ -1895,21 +1841,7 @@ fun equal_prod A_ B_ = {equal = equal_proda A_ B_} : ('a * 'b) HOL.equal;
 
 end; (*struct Product_Type*)
 
-structure CDCL_W_Level : sig
-  val get_maximum_level :
-    'a HOL.equal ->
-      ('a, 'b) Partial_Annotated_Clausal_Logic.ann_lit list ->
-        'a Clausal_Logic.literal Multiset.multiset -> Arith.nat
-  val do_backtrack_step :
-    'a HOL.equal ->
-      ('a, ('a Clausal_Logic.literal list))
-        Partial_Annotated_Clausal_Logic.ann_lit list *
-        ('b * (('a Clausal_Logic.literal list) list *
-                (Arith.nat * ('a Clausal_Logic.literal list) option))) ->
-        ('a, ('a Clausal_Logic.literal list))
-          Partial_Annotated_Clausal_Logic.ann_lit list *
-          ('b * (('a Clausal_Logic.literal list) list *
-                  (Arith.nat * ('a Clausal_Logic.literal list) option)))
+structure DPLL_CDCL_W_Implementation : sig
   val find_first_unused_var :
     'a HOL.equal ->
       ('a Clausal_Logic.literal list) list ->
@@ -1917,43 +1849,16 @@ structure CDCL_W_Level : sig
   val find_first_unit_clause :
     'a HOL.equal ->
       ('a Clausal_Logic.literal list) list ->
-        ('a, 'b) Partial_Annotated_Clausal_Logic.ann_lit list ->
+        ('a, 'b, 'c) Partial_Annotated_Clausal_Logic.ann_lit list ->
           ('a Clausal_Logic.literal * 'a Clausal_Logic.literal list) option
 end = struct
-
-fun maximum_level_code A_ [] uu = Arith.Zero_nat
-  | maximum_level_code A_ (l :: ls) m =
-    Orderings.max Arith.ord_nat
-      (List.size_list
-        (List.filter Partial_Annotated_Clausal_Logic.is_decided
-          (List.dropWhile
-            (fn s =>
-              not (HOL.eq A_
-                    (Clausal_Logic.atm_of
-                      (Partial_Annotated_Clausal_Logic.lit_of s))
-                    (Clausal_Logic.atm_of l)))
-            m)))
-      (maximum_level_code A_ ls m);
-
-fun get_maximum_level A_ m (Multiset.Mset d) = maximum_level_code A_ d m;
-
-fun bt_cut i (Partial_Annotated_Clausal_Logic.Propagated (uu, uv) :: ls) =
-  bt_cut i ls
-  | bt_cut i (Partial_Annotated_Clausal_Logic.Decided k :: ls) =
-    (if Arith.equal_nata
-          (List.size_list
-            (List.filter Partial_Annotated_Clausal_Logic.is_decided ls))
-          i
-      then SOME (Partial_Annotated_Clausal_Logic.Decided k :: ls)
-      else bt_cut i ls)
-  | bt_cut i [] = NONE;
 
 fun is_unit_clause_code A_ l m =
   (case List.filter
           (fn a =>
             not (Set.member A_ (Clausal_Logic.atm_of a)
                   (Set.image Clausal_Logic.atm_of
-                    (Partial_Annotated_Clausal_Logic.lits_of (Set.Set m)))))
+                    (Partial_Annotated_Clausal_Logic.lits_of m))))
           l
     of [] => NONE
     | [a] =>
@@ -1961,44 +1866,12 @@ fun is_unit_clause_code A_ l m =
             (fn c =>
               Set.member (Clausal_Logic.equal_literal A_)
                 (Clausal_Logic.uminus_literal c)
-                (Partial_Annotated_Clausal_Logic.lits_of (Set.Set m)))
+                (Partial_Annotated_Clausal_Logic.lits_of m))
             (List.remove1 (Clausal_Logic.equal_literal A_) a l)
         then SOME a else NONE)
     | _ :: _ :: _ => NONE);
 
 fun is_unit_clause A_ l m = is_unit_clause_code A_ l m;
-
-fun find_level_decomp A_ m [] d k = NONE
-  | find_level_decomp A_ m (l :: ls) d k =
-    let
-      val (i, j) =
-        (List.size_list
-           (List.filter Partial_Annotated_Clausal_Logic.is_decided
-             (List.dropWhile
-               (fn s =>
-                 not (HOL.eq A_
-                       (Clausal_Logic.atm_of
-                         (Partial_Annotated_Clausal_Logic.lit_of s))
-                       (Clausal_Logic.atm_of l)))
-               m)),
-          maximum_level_code A_ (d @ ls) m);
-    in
-      (if Arith.equal_nata i k andalso Arith.less_nat j i then SOME (l, j)
-        else find_level_decomp A_ m ls (l :: d) k)
-    end;
-
-fun do_backtrack_step A_ (m, (n, (u, (k, SOME d)))) =
-  (case find_level_decomp A_ m d [] k of NONE => (m, (n, (u, (k, SOME d))))
-    | SOME (l, j) =>
-      (case bt_cut j m of NONE => (m, (n, (u, (k, SOME d))))
-        | SOME [] => (m, (n, (u, (k, SOME d))))
-        | SOME (Partial_Annotated_Clausal_Logic.Decided _ :: ls) =>
-          (Partial_Annotated_Clausal_Logic.Propagated (l, d) :: ls,
-            (n, (d :: u, (j, NONE))))
-        | SOME (Partial_Annotated_Clausal_Logic.Propagated (_, _) :: _) =>
-          (m, (n, (u, (k, SOME d))))))
-  | do_backtrack_step A_ (v, (vb, (vd, (vf, NONE)))) =
-    (v, (vb, (vd, (vf, NONE))));
 
 fun find_first_unused_var A_ (a :: l) m =
   (case List.find
@@ -2015,37 +1888,36 @@ fun find_first_unit_clause A_ (a :: l) m =
     | SOME la => SOME (la, a))
   | find_first_unit_clause A_ [] uu = NONE;
 
-end; (*struct CDCL_W_Level*)
+end; (*struct DPLL_CDCL_W_Implementation*)
 
 structure CDCL_W_Implementation : sig
-  datatype 'a cdcl_W_state_inv_from_init_state =
+  datatype cdcl_W_state_inv_from_init_state =
     ConI of
-      (('a, ('a Clausal_Logic.literal list))
+      ((Arith.nat, Arith.nat, (Arith.nat Clausal_Logic.literal list))
          Partial_Annotated_Clausal_Logic.ann_lit list *
-        (('a Clausal_Logic.literal list) list *
-          (('a Clausal_Logic.literal list) list *
-            (Arith.nat * ('a Clausal_Logic.literal list) option))))
+        ((Arith.nat Clausal_Logic.literal list) list *
+          ((Arith.nat Clausal_Logic.literal list) list *
+            (Arith.nat * (Arith.nat Clausal_Logic.literal list) option))));
   val gene : Arith.nat -> (Arith.nat Clausal_Logic.literal list) list
   val do_all_cdcl_W_stgy :
-    'a HOL.equal ->
-      'a cdcl_W_state_inv_from_init_state -> 'a cdcl_W_state_inv_from_init_state
+    cdcl_W_state_inv_from_init_state -> cdcl_W_state_inv_from_init_state
 end = struct
 
-datatype 'a cdcl_W_state_inv =
+datatype cdcl_W_state_inv =
   Con of
-    (('a, ('a Clausal_Logic.literal list))
+    ((Arith.nat, Arith.nat, (Arith.nat Clausal_Logic.literal list))
        Partial_Annotated_Clausal_Logic.ann_lit list *
-      (('a Clausal_Logic.literal list) list *
-        (('a Clausal_Logic.literal list) list *
-          (Arith.nat * ('a Clausal_Logic.literal list) option))));
+      ((Arith.nat Clausal_Logic.literal list) list *
+        ((Arith.nat Clausal_Logic.literal list) list *
+          (Arith.nat * (Arith.nat Clausal_Logic.literal list) option))));
 
-datatype 'a cdcl_W_state_inv_from_init_state =
+datatype cdcl_W_state_inv_from_init_state =
   ConI of
-    (('a, ('a Clausal_Logic.literal list))
+    ((Arith.nat, Arith.nat, (Arith.nat Clausal_Logic.literal list))
        Partial_Annotated_Clausal_Logic.ann_lit list *
-      (('a Clausal_Logic.literal list) list *
-        (('a Clausal_Logic.literal list) list *
-          (Arith.nat * ('a Clausal_Logic.literal list) option))));
+      ((Arith.nat Clausal_Logic.literal list) list *
+        ((Arith.nat Clausal_Logic.literal list) list *
+          (Arith.nat * (Arith.nat Clausal_Logic.literal list) option))));
 
 fun gene Arith.Zero_nat =
   [[Clausal_Logic.Pos Arith.Zero_nat], [Clausal_Logic.Neg Arith.Zero_nat]]
@@ -2053,10 +1925,18 @@ fun gene Arith.Zero_nat =
     List.map (fn a => Clausal_Logic.Pos (Arith.Suc n) :: a) (gene n) @
       List.map (fn a => Clausal_Logic.Neg (Arith.Suc n) :: a) (gene n);
 
+fun bt_cut i (Partial_Annotated_Clausal_Logic.Propagated (uu, uv) :: ls) =
+  bt_cut i ls
+  | bt_cut i (Partial_Annotated_Clausal_Logic.Decided (ka, k) :: ls) =
+    (if Arith.equal_nata k (Arith.Suc i)
+      then SOME (Partial_Annotated_Clausal_Logic.Decided (ka, k) :: ls)
+      else bt_cut i ls)
+  | bt_cut i [] = NONE;
+
 fun do_propagate_step A_ s =
   (case s
     of (m, (n, (u, (k, NONE)))) =>
-      (case CDCL_W_Level.find_first_unit_clause A_ (n @ u) m
+      (case DPLL_CDCL_W_Implementation.find_first_unit_clause A_ (n @ u) m
         of NONE => (m, (n, (u, (k, NONE))))
         | SOME (l, c) =>
           (Partial_Annotated_Clausal_Logic.Propagated (l, c) :: m,
@@ -2069,7 +1949,7 @@ fun find_conflict A_ m [] = NONE
           (fn c =>
             Set.member (Clausal_Logic.equal_literal A_)
               (Clausal_Logic.uminus_literal c)
-              (Partial_Annotated_Clausal_Logic.lits_of (Set.Set m)))
+              (Partial_Annotated_Clausal_Logic.lits_of m))
           n
       then SOME n else find_conflict A_ m ns);
 
@@ -2088,181 +1968,227 @@ fun id_of_I_to s = Con (rough_state_from_init_state_of s);
 
 fun rough_state_of (Con x) = x;
 
-fun do_cp_stepa A_ s = Con (do_cp_step A_ (rough_state_of s));
+fun do_cp_stepa s = Con (do_cp_step Arith.equal_nat (rough_state_of s));
 
-fun do_skip_step A_
+fun do_skip_step
   (Partial_Annotated_Clausal_Logic.Propagated (l, c) :: ls,
     (n, (u, (k, SOME d))))
-  = (if not (List.member (Clausal_Logic.equal_literal A_) d
+  = (if not (List.member (Clausal_Logic.equal_literal Arith.equal_nat) d
               (Clausal_Logic.uminus_literal l)) andalso
           not (List.null d)
       then (ls, (n, (u, (k, SOME d))))
       else (Partial_Annotated_Clausal_Logic.Propagated (l, c) :: ls,
              (n, (u, (k, SOME d)))))
-  | do_skip_step A_ ([], va) = ([], va)
-  | do_skip_step A_ (Partial_Annotated_Clausal_Logic.Decided vd :: vc, va) =
-    (Partial_Annotated_Clausal_Logic.Decided vd :: vc, va)
-  | do_skip_step A_ (v, (vb, (vd, (vf, NONE)))) = (v, (vb, (vd, (vf, NONE))));
+  | do_skip_step ([], va) = ([], va)
+  | do_skip_step (Partial_Annotated_Clausal_Logic.Decided (vd, ve) :: vc, va) =
+    (Partial_Annotated_Clausal_Logic.Decided (vd, ve) :: vc, va)
+  | do_skip_step (v, (vb, (vd, (vf, NONE)))) = (v, (vb, (vd, (vf, NONE))));
 
-fun do_resolve_step A_
+fun maximum_level_code A_ d m =
+  CDCL_W_Level.get_maximum_level A_ m (Multiset.Mset d);
+
+fun find_level_decomp A_ m [] d k = NONE
+  | find_level_decomp A_ m (l :: ls) d k =
+    let
+      val (i, j) =
+        (CDCL_W_Level.get_rev_level A_ (List.rev m) Arith.Zero_nat l,
+          maximum_level_code A_ (d @ ls) m);
+    in
+      (if Arith.equal_nata i k andalso Arith.less_nat j i then SOME (l, j)
+        else find_level_decomp A_ m ls (l :: d) k)
+    end;
+
+fun do_backtrack_step A_ (m, (n, (u, (k, SOME d)))) =
+  (case find_level_decomp A_ m d [] k of NONE => (m, (n, (u, (k, SOME d))))
+    | SOME (l, j) =>
+      (case bt_cut j m of NONE => (m, (n, (u, (k, SOME d))))
+        | SOME [] => (m, (n, (u, (k, SOME d))))
+        | SOME (Partial_Annotated_Clausal_Logic.Decided (_, _) :: ls) =>
+          (Partial_Annotated_Clausal_Logic.Propagated (l, d) :: ls,
+            (n, (d :: u, (j, NONE))))
+        | SOME (Partial_Annotated_Clausal_Logic.Propagated (_, _) :: _) =>
+          (m, (n, (u, (k, SOME d))))))
+  | do_backtrack_step A_ (v, (vb, (vd, (vf, NONE)))) =
+    (v, (vb, (vd, (vf, NONE))));
+
+fun do_resolve_step
   (Partial_Annotated_Clausal_Logic.Propagated (l, c) :: ls,
     (n, (u, (k, SOME d))))
-  = (if List.member (Clausal_Logic.equal_literal A_) d
+  = (if List.member (Clausal_Logic.equal_literal Arith.equal_nat) d
           (Clausal_Logic.uminus_literal l) andalso
           Arith.equal_nata
-            (CDCL_W_Level.get_maximum_level A_
-              (Partial_Annotated_Clausal_Logic.Propagated (l, c) :: ls)
-              (Multiset.Mset
-                (List.remove1 (Clausal_Logic.equal_literal A_)
-                  (Clausal_Logic.uminus_literal l) d)))
+            (maximum_level_code Arith.equal_nat
+              (List.remove1 (Clausal_Logic.equal_literal Arith.equal_nat)
+                (Clausal_Logic.uminus_literal l) d)
+              (Partial_Annotated_Clausal_Logic.Propagated (l, c) :: ls))
             k
-      then (ls, (n, (u, (k, SOME (List.remdups (Clausal_Logic.equal_literal A_)
+      then (ls, (n, (u, (k, SOME (List.remdups
+                                   (Clausal_Logic.equal_literal Arith.equal_nat)
                                    (List.remove1
-                                      (Clausal_Logic.equal_literal A_) l c @
+                                      (Clausal_Logic.equal_literal
+Arith.equal_nat)
+                                      l c @
                                      List.remove1
-                                       (Clausal_Logic.equal_literal A_)
+                                       (Clausal_Logic.equal_literal
+ Arith.equal_nat)
                                        (Clausal_Logic.uminus_literal l) d))))))
       else (Partial_Annotated_Clausal_Logic.Propagated (l, c) :: ls,
              (n, (u, (k, SOME d)))))
-  | do_resolve_step A_ ([], va) = ([], va)
-  | do_resolve_step A_ (Partial_Annotated_Clausal_Logic.Decided vd :: vc, va) =
-    (Partial_Annotated_Clausal_Logic.Decided vd :: vc, va)
-  | do_resolve_step A_ (v, (vb, (vd, (vf, NONE)))) =
-    (v, (vb, (vd, (vf, NONE))));
+  | do_resolve_step ([], va) = ([], va)
+  | do_resolve_step (Partial_Annotated_Clausal_Logic.Decided (vd, ve) :: vc, va)
+    = (Partial_Annotated_Clausal_Logic.Decided (vd, ve) :: vc, va)
+  | do_resolve_step (v, (vb, (vd, (vf, NONE)))) = (v, (vb, (vd, (vf, NONE))));
 
-fun do_decide_step A_ (D1_, D2_) (m, (n, (u, (k, NONE)))) =
-  (case CDCL_W_Level.find_first_unused_var A_ n
-          (Partial_Annotated_Clausal_Logic.lits_of (Set.Set m))
+fun do_decide_step A_ (m, (n, (u, (k, NONE)))) =
+  (case DPLL_CDCL_W_Implementation.find_first_unused_var A_ n
+          (Partial_Annotated_Clausal_Logic.lits_of m)
     of NONE => (m, (n, (u, (k, NONE))))
     | SOME l =>
-      (Partial_Annotated_Clausal_Logic.Decided l :: m,
-        (n, (u, (Arith.plus D2_ k (Arith.one D1_), NONE)))))
-  | do_decide_step A_ (D1_, D2_) (v, (vb, (vd, (vf, SOME vh)))) =
+      (Partial_Annotated_Clausal_Logic.Decided (l, Arith.Suc k) :: m,
+        (n, (u, (Arith.plus_nat k Arith.one_nat, NONE)))))
+  | do_decide_step A_ (v, (vb, (vd, (vf, SOME vh)))) =
     (v, (vb, (vd, (vf, SOME vh))));
 
-fun do_other_step A_ s =
+fun do_other_step s =
   let
-    val t = do_skip_step A_ s;
+    val t = do_skip_step s;
   in
     (if not (Product_Type.equal_proda
               (List.equal_list
-                (Partial_Annotated_Clausal_Logic.equal_ann_lit A_
-                  (List.equal_list (Clausal_Logic.equal_literal A_))))
+                (Partial_Annotated_Clausal_Logic.equal_ann_lit
+                  Arith.equal_nat Arith.equal_nat
+                  (List.equal_list
+                    (Clausal_Logic.equal_literal Arith.equal_nat))))
               (Product_Type.equal_prod
                 (List.equal_list
-                  (List.equal_list (Clausal_Logic.equal_literal A_)))
+                  (List.equal_list
+                    (Clausal_Logic.equal_literal Arith.equal_nat)))
                 (Product_Type.equal_prod
                   (List.equal_list
-                    (List.equal_list (Clausal_Logic.equal_literal A_)))
+                    (List.equal_list
+                      (Clausal_Logic.equal_literal Arith.equal_nat)))
                   (Product_Type.equal_prod Arith.equal_nat
                     (Option.equal_option
-                      (List.equal_list (Clausal_Logic.equal_literal A_))))))
+                      (List.equal_list
+                        (Clausal_Logic.equal_literal Arith.equal_nat))))))
               t s)
       then t
       else let
-             val u = do_resolve_step A_ t;
+             val u = do_resolve_step t;
            in
              (if not (Product_Type.equal_proda
                        (List.equal_list
-                         (Partial_Annotated_Clausal_Logic.equal_ann_lit A_
-                           (List.equal_list (Clausal_Logic.equal_literal A_))))
+                         (Partial_Annotated_Clausal_Logic.equal_ann_lit
+                           Arith.equal_nat Arith.equal_nat
+                           (List.equal_list
+                             (Clausal_Logic.equal_literal Arith.equal_nat))))
                        (Product_Type.equal_prod
                          (List.equal_list
-                           (List.equal_list (Clausal_Logic.equal_literal A_)))
+                           (List.equal_list
+                             (Clausal_Logic.equal_literal Arith.equal_nat)))
                          (Product_Type.equal_prod
                            (List.equal_list
-                             (List.equal_list (Clausal_Logic.equal_literal A_)))
+                             (List.equal_list
+                               (Clausal_Logic.equal_literal Arith.equal_nat)))
                            (Product_Type.equal_prod Arith.equal_nat
                              (Option.equal_option
                                (List.equal_list
-                                 (Clausal_Logic.equal_literal A_))))))
+                                 (Clausal_Logic.equal_literal
+                                   Arith.equal_nat))))))
                        u t)
                then u
                else let
-                      val v = CDCL_W_Level.do_backtrack_step A_ u;
+                      val v = do_backtrack_step Arith.equal_nat u;
                     in
                       (if not (Product_Type.equal_proda
                                 (List.equal_list
                                   (Partial_Annotated_Clausal_Logic.equal_ann_lit
-                                    A_ (List.equal_list
- (Clausal_Logic.equal_literal A_))))
+                                    Arith.equal_nat Arith.equal_nat
+                                    (List.equal_list
+                                      (Clausal_Logic.equal_literal
+Arith.equal_nat))))
                                 (Product_Type.equal_prod
                                   (List.equal_list
                                     (List.equal_list
-                                      (Clausal_Logic.equal_literal A_)))
+                                      (Clausal_Logic.equal_literal
+Arith.equal_nat)))
                                   (Product_Type.equal_prod
                                     (List.equal_list
                                       (List.equal_list
-(Clausal_Logic.equal_literal A_)))
+(Clausal_Logic.equal_literal Arith.equal_nat)))
                                     (Product_Type.equal_prod Arith.equal_nat
                                       (Option.equal_option
-(List.equal_list (Clausal_Logic.equal_literal A_))))))
+(List.equal_list (Clausal_Logic.equal_literal Arith.equal_nat))))))
                                 v u)
-                        then v
-                        else do_decide_step A_ (Arith.one_nat, Arith.plus_nat)
-                               v)
+                        then v else do_decide_step Arith.equal_nat v)
                     end)
            end)
   end;
 
-fun do_other_stepa A_ s = Con (do_other_step A_ (rough_state_of s));
+fun do_other_stepa s = Con (do_other_step (rough_state_of s));
 
-fun equal_cdcl_W_state_inv A_ sa s =
+fun equal_cdcl_W_state_inv sa s =
   Product_Type.equal_proda
     (List.equal_list
-      (Partial_Annotated_Clausal_Logic.equal_ann_lit A_
-        (List.equal_list (Clausal_Logic.equal_literal A_))))
+      (Partial_Annotated_Clausal_Logic.equal_ann_lit Arith.equal_nat
+        Arith.equal_nat
+        (List.equal_list (Clausal_Logic.equal_literal Arith.equal_nat))))
     (Product_Type.equal_prod
-      (List.equal_list (List.equal_list (Clausal_Logic.equal_literal A_)))
+      (List.equal_list
+        (List.equal_list (Clausal_Logic.equal_literal Arith.equal_nat)))
       (Product_Type.equal_prod
-        (List.equal_list (List.equal_list (Clausal_Logic.equal_literal A_)))
+        (List.equal_list
+          (List.equal_list (Clausal_Logic.equal_literal Arith.equal_nat)))
         (Product_Type.equal_prod Arith.equal_nat
           (Option.equal_option
-            (List.equal_list (Clausal_Logic.equal_literal A_))))))
+            (List.equal_list (Clausal_Logic.equal_literal Arith.equal_nat))))))
     (rough_state_of sa) (rough_state_of s);
 
-fun do_full1_cp_step A_ s =
+fun do_full1_cp_step s =
   let
-    val sa = do_cp_stepa A_ s;
+    val sa = do_cp_stepa s;
   in
-    (if equal_cdcl_W_state_inv A_ s sa then s else do_full1_cp_step A_ sa)
+    (if equal_cdcl_W_state_inv s sa then s else do_full1_cp_step sa)
   end;
 
-fun equal_cdcl_W_state_inv_from_init_state A_ sa s =
+fun equal_cdcl_W_state_inv_from_init_state sa s =
   Product_Type.equal_proda
     (List.equal_list
-      (Partial_Annotated_Clausal_Logic.equal_ann_lit A_
-        (List.equal_list (Clausal_Logic.equal_literal A_))))
+      (Partial_Annotated_Clausal_Logic.equal_ann_lit Arith.equal_nat
+        Arith.equal_nat
+        (List.equal_list (Clausal_Logic.equal_literal Arith.equal_nat))))
     (Product_Type.equal_prod
-      (List.equal_list (List.equal_list (Clausal_Logic.equal_literal A_)))
+      (List.equal_list
+        (List.equal_list (Clausal_Logic.equal_literal Arith.equal_nat)))
       (Product_Type.equal_prod
-        (List.equal_list (List.equal_list (Clausal_Logic.equal_literal A_)))
+        (List.equal_list
+          (List.equal_list (Clausal_Logic.equal_literal Arith.equal_nat)))
         (Product_Type.equal_prod Arith.equal_nat
           (Option.equal_option
-            (List.equal_list (Clausal_Logic.equal_literal A_))))))
+            (List.equal_list (Clausal_Logic.equal_literal Arith.equal_nat))))))
     (rough_state_from_init_state_of sa) (rough_state_from_init_state_of s);
 
-fun do_cdcl_W_stgy_step A_ s =
+fun do_cdcl_W_stgy_step s =
   let
-    val t = do_full1_cp_step A_ s;
+    val t = do_full1_cp_step s;
   in
-    (if not (equal_cdcl_W_state_inv A_ t s) then t
+    (if not (equal_cdcl_W_state_inv t s) then t
       else let
-             val a = do_other_stepa A_ t;
+             val a = do_other_stepa t;
            in
-             do_full1_cp_step A_ a
+             do_full1_cp_step a
            end)
   end;
 
-fun do_cdcl_W_stgy_stepa A_ s =
-  ConI (rough_state_of (do_cdcl_W_stgy_step A_ (id_of_I_to s)));
+fun do_cdcl_W_stgy_stepa s =
+  ConI (rough_state_of (do_cdcl_W_stgy_step (id_of_I_to s)));
 
-fun do_all_cdcl_W_stgy A_ s =
+fun do_all_cdcl_W_stgy s =
   let
-    val t = do_cdcl_W_stgy_stepa A_ s;
+    val t = do_cdcl_W_stgy_stepa s;
   in
-    (if equal_cdcl_W_state_inv_from_init_state A_ t s then s
-      else do_all_cdcl_W_stgy A_ t)
+    (if equal_cdcl_W_state_inv_from_init_state t s then s
+      else do_all_cdcl_W_stgy t)
   end;
 
 end; (*struct CDCL_W_Implementation*)
@@ -2274,12 +2200,12 @@ open CDCL_W_Implementation;
 open Arith;
 let
   val N = gene (Suc (Suc (Suc (((Suc Zero_nat))))))
-  val f = do_all_cdcl_W_stgy equal_nat
-    (CDCL_W_Implementation.ConI ([], (N, ([], (Zero_nat, NONE)))))
+  val f = do_all_cdcl_W_stgy (CDCL_W_Implementation.ConI ([], (N, ([], (Zero_nat, NONE)))))
   in
+
   f
 end
 \<close>
-(*>*)
 
+(*>*)
 end
